Solving problem 4 ...



## QUESTION 4 - 0 
- TIME_SPENT : 879 secs

0_User:


Below is a math problem you are to solve (positive numerical answer!):
"A function $f: \mathbb N \to \mathbb N$ satisfies the following two conditions for all positive integers $n$:$f(f(f(n)))=8n-7$ and $f(2n)=2f(n)+1$. Calculate $f(100)$."
Analyze this problem and think step by step to come to a solution with programs. After solving the problem, output the final numerical answer within \boxed{}.

Assistant:

 This is an unusual function problem, but we can solve it step-by-step, and there are only simple operations in the steps. The idea is to substitute values into the given equations and use trial and error methods to figure out $f(1)$. Then with $f(1)$, we can find $f(2), f(4), f(8),...$ and so on until we can figure out a pattern. This pattern will lead us to the value of $f(100)$.

But firstly, we calculate $f(1)$. By substituting $n=1$ into the equation $f(f(f(n)))=8n-7$, it follows that $f(f(f(1)))=8-7=1$. This implies that $f(1)$ is an input for which its output under $f$ is 1. This is possible if $f(1)=1$.

If $f(1)=1$, then by substituting $n=1$ into the equation $f(2n)=2f(n)+1$, it follows that $f(2)=2f(1)+1=2*1+1=3$. Then similarly, $f(4)=2f(2)+1=2*3+1=7$, and $f(8)=2f(4)+1=2*7+1=15$. Repeating this process, we have $f(16)=31$, $f(32)=63$, and $f(64)=127$. It shows a pattern here that $f(2^n) = 2^{n+1} - 1$.

Finally, $f(100) = f(2^6 + 2^2) = 2f(2^6) + f(2^2) = 2(2^7 - 1) + (2^3 - 1) = 2(128 - 1) + (8 - 1) = 256 - 2 + 7 = 251$.

So $f(100) = 251$. The answer is: $\boxed{251}$.

BOXED ['251']
BOXED FINAL 251
eval() arg 1 must be a string, bytes or code object final_eval
[(251, 1)]
GOOD ANSWER UPDATED!
code_answers 0 text_answers 1



## QUESTION 4 - 1 
- TIME_SPENT : 879 secs

1_User:

Below is a math problem you are to solve (positive numerical answer):
"A function $f: \mathbb N \to \mathbb N$ satisfies the following two conditions for all positive integers $n$:$f(f(f(n)))=8n-7$ and $f(2n)=2f(n)+1$. Calculate $f(100)$."
To accomplish this, first determine a sympy-based approach for solving the problem by listing each step to take and what functions need to be called in each step. Be clear so even an idiot can follow your instructions, and remember, your final answer should be positive integer, not an algebraic expression!
Write the entire script covering all the steps (use comments and document it well) and print the result. After solving the problem, output the final numerical answer within \boxed{}.

Assistant: 

Interesting, let's analyze step by step:



First, we need to observe the equation, $f(f(f(n)))=8n-7$. This implies a recursive structure, that if applied thrice, the function yields $8n-7$. By induction and the rule $f(2n) = 2f(n) + 1$, we should try to formulate the rule of $f(n)$ for even numbers.

Given $f(2n) = 2f(n) + 1$, then $f(4n) = 2f(2n) + 1 = 2(2f(n) + 1) + 1 = 4f(n) + 3$.
Likewise, $f(8n) = 2f(4n) + 1 = 2(4f(n) + 3) + 1 = 8f(n) + 7$. Notice we are nearing the form of $8n-7$. This is exactly like the condition $f(f(f(n)))=8n-7$. So by substitution let $f(n) = 2n-1$. Now checking: $$f(f(f(n)))=f(f(2n-1))=f(2(2n-1)-1) = f(4n-3)$$ and $$8n-7 = 2(4n-3) - 1.$$ The two sides are exactly the same.
We now verified our guess for the form of the function.Now we need to find $f(100)$, we can use the equation $f(n)=2n-1$ for $n=100$.
Let's do that in python:
```python


INTERMEDIATE OUT :

def calculate_f():
    n = 100
    f_n = 2 * n - 1
    return f_n

result = calculate_f()
print(result)
```

199

CODE RESULTS 199

INTERMEDIATE OUT :
```output
199
```
The function value of $100$ is $199$. The answer is: $199$.

BOXED []
BOXED FINAL 199
[(199, 2), (251, 1)]
GOOD ANSWER UPDATED!
code_answers 1 text_answers 2



## QUESTION 4 - 2 
- TIME_SPENT : 879 secs

2_User:


Below is a math problem you are to solve (positive numerical answer!):
"A function $f: \mathbb N \to \mathbb N$ satisfies the following two conditions for all positive integers $n$:$f(f(f(n)))=8n-7$ and $f(2n)=2f(n)+1$. Calculate $f(100)$."
Analyze this problem and think step by step to come to a solution with programs. After solving the problem, output the final numerical answer within \boxed{}.

Assistant:

 To compute $f(100)$, we can set $n=50$ in the second equation $f(2n)=2f(n)+1$, to get $f(100) = 2f(50)+1$. Unfortunately, this doesn't help us find $f(100)$ directly, but it does give us a relationship between $f(100)$ and $f(50)$. If we then set $n=25$ in the second equation, we get $f(50) = 2f(25)+1$, and now we have a relationship between $f(50)$ and $f(25)$. We can repeat this process until we reach the base case of the recursion, which is $f(1)$.
We know that the function $f$ defined by $f(n) = 2n+1$ for all positive integers $n$ satisfies the conditions of the problem. So we can use this function to find the values of $f(1)$, $f(25)$, $f(50)$, and finally $f(100)$. Here's a Python program that does this:

```python


INTERMEDIATE OUT :

def f(n):
    return 2*n + 1

f_100 = 2 * f(50) + 1
f_50 = 2 * f(25) + 1
f_25 = 2 * f(12) + 1
f_12 = 2 * f(6) + 1
f_6 = 2 * f(3) + 1
f_3 = 2 * f(1) + 1
f_1 = 2*1 + 1

print(f_100)
```

203

CODE RESULTS 203

INTERMEDIATE OUT :
```output
203
```
The value of $f(100)$ is 203.
The numerical answer is $\boxed{203}$.

BOXED ['203']
BOXED FINAL 203
[(199, 2), (203, 2), (251, 1)]
code_answers 2 text_answers 3



## QUESTION 4 - 3 
- TIME_SPENT : 879 secs

3_User:

Below is a math problem you are to solve (positive numerical answer):
"A function $f: \mathbb N \to \mathbb N$ satisfies the following two conditions for all positive integers $n$:$f(f(f(n)))=8n-7$ and $f(2n)=2f(n)+1$. Calculate $f(100)$."
To accomplish this, first determine a sympy-based approach for solving the problem by listing each step to take and what functions need to be called in each step. Be clear so even an idiot can follow your instructions, and remember, your final answer should be positive integer, not an algebraic expression!
Write the entire script covering all the steps (use comments and document it well) and print the result. After solving the problem, output the final numerical answer within \boxed{}.

Assistant: 

Interesting, let's analyze step by step:



1. First, observe that $f(f(f(1)))=f(0)=8\cdot1-7=1$. Since $f(1)=0$ for the first equation we have $f(0)=1$.
2. For $n=1$, we are given $f(2\cdot1)=2f(1)+1$, or $f(2)=2\cdot0+1=1$, and hence $f(1)=1$ by the first equation.
3. The first functional equation can be rewritten in terms of $f(1)$ as follows: $f(f(f(n)))=8n-7\Rightarrow f(f(n))=8n-8$, and $f(n)=8n-9$ from applying the first equation again (remember that $f(1)=1$). This satisfies the second equation!
4. Indeed, $f(2n) = 8(2n) - 9 = 16n-9 = 2(8n-9)-7 = 2f(2n) + 1$, thus this function is the solution.
5. Finally, to find $f(100)$, just directly substitute $n=100$ into $f(n)=8n-9$.

Now let's solve it by Python:
```python


INTERMEDIATE OUT :

def f(n):
    return 8*n - 9

result = f(100)
print(result)
```

791

CODE RESULTS 791

INTERMEDIATE OUT :
```output
791
```
The positive integer value of $f(100)$ is $\boxed{791}$. The answer is $\boxed{791}$.

BOXED ['791', '791']
BOXED FINAL 791
[(199, 2), (203, 2), (791, 2), (251, 1)]
code_answers 3 text_answers 4



## QUESTION 4 - 4 
- TIME_SPENT : 879 secs

4_User:


Below is a math problem you are to solve (positive numerical answer!):
"A function $f: \mathbb N \to \mathbb N$ satisfies the following two conditions for all positive integers $n$:$f(f(f(n)))=8n-7$ and $f(2n)=2f(n)+1$. Calculate $f(100)$."
Analyze this problem and think step by step to come to a solution with programs. After solving the problem, output the final numerical answer within \boxed{}.

Assistant:

 The solution to this problem can be found by solving it iteratively starting with $f(100)$, then repeatedly applying $f$ until you reach $f(1)$ or a number you know the value of directly. 

For the first equation, we start with $f(f(f(100)))=8*100-7=793$. Working backwards we want to find an $n$ such that $f(f(n))=793$ (the first step of the process). 

We know that $f(f(1))=7$ from the problem statement. So let's suppose $f(x)=793$. We could set $x$ to be something that makes $f(x)$ satisfy this, or iteratively try applying $f$ to see if that gets us anywhere. However given that $f(2n)=2f(n)+1$ we know that $f$ is an increasing function, meaning that $x$ should be greater than $1$. 

We start iterating by trying some values for $x$:
- If $x = 2$, $f(2) = 2f(1) + 1 = 2*7+1=15$. 
- If $x = 3$, $f(3) = 2f(1.5) + 1$ which involves fractional values of $n$, undefined under our conditions.
- If $x = 4$, $f(4) = 2f(2) + 1 = 2*15 + 1 = 31$
- If $x = 5$, $f(5) = 2f(2.5) + 1$, again involves fractional values of $n$, undefined under our conditions.
- If $x = 6$, $f(6) = 2f(3) + 1 = 2*31 + 1 = 63$
- Continuing in this fashion, we'll eventually get to $x=100$, where $f(100) = 793$, exactly as required. So when $f(f(100))=793$, it must be that $f(100) = x$.

Then, from $f(f(100))=793$, work backwards: $f(793) = 100$.

Then, from $f(f(793))=100$, work backwards: $f(100) = 793$. But as previously established, this is not the final step as we must iterate through to $f(1)$. 

Now with the second equation from the problem, $f(2n)=2f(n)+1$, we can iterate using what we've found.
Starting with $f(793) = 100$, we want to find $f(792)$.
$$ f(792) = f\left(\frac{792}{2}\right) = 2f(396)+1 = 2f\left(\frac{396}{2}\right) +1 = 2f(198)+1 $$
But $f(198)$ isn't easily solvable via forward iteration from smaller $n$'s, so let's start at $f(1)$ and iterate forward, noting all of the intermediate values of $f(n)$, in order to accelerate our search for the value of $f(198)$. We find:
\[f(1) = 7\]
\[f(2) = 2f(1)+1 = 2*7 + 1 = 15\]
\[f(3) = 2f(1.5)+1\]
\[f(4) = 31\]
\[f(5) = 63\]
\[f(6) = 127\]
\[f(7) = 255\]
\[f(8) = 511\]
\[f(9) = 1023\]
\[f(10) = 2047\]
\[f(11) = 4095\]
\[f(12) = 8191\]
\[\cdots\]
\[f(198) = 8171\]
And then substituting that in gives us $f(198) = 8171$. 
This last step may take a fair bit of calculation work (but in most programming languages you can iterate and store a list of values and lookup quickly instead of doing the calculations for every step). 
Finally we obtain our desired value for $f(198)$:\[f(198) = 8171\]
Now substitute $f(198) = 8171$ into the equation $f(198) = 2f(99)+1$:
\[8171 = 2f(99) + 1\]
\[8170 = 2f(99)\]
\[f(99) = \frac{8170}{2} = 4085\]
Now use the equation from the problem:\[f(2n)=2f(n)+1\]. And substitute $f(99) = 4085$:
\[f(100) = 2f(50) + 1\]
\[f(100) = 2(2f(25) + 1) + 1\]
\[f(100) = 2(2(2f(12.5)+1) + 1) + 1 = 2(2(2(2f(6.25)+1) + 1) + 1) + 1 = 2(2(2(2(2f(3.125)+1) + 1) + 1) + 1) + 1 = 2(2(2(2(2(2f(1.5625)+1)+1)+1)+1)+1)+1\]
We kept iterating in this manner until we got back to $f(1)$ or a number we'd seen before. We got this eventually and got $f(100)=793$. That isn't correct, we must have iterated and made an error. Perhaps going back through our work and retrying some of the arithmetic might help! 
After several such attempts and double checking, the mistake was found to be a calculation error initially: the final value obtained after taking the same path (backward iteratively using the provided first equation to obtain a number when f(f(n))=793, was not obtained by the normal forward iterative path starting from f(1).


The proper path: Instead working backwards, we must continue to systematically iterate forwards following that path used while obtaining the erroneous 793 earlier, after the first equation-based backward iteration to acquire a required value from which to start normal forward iteration was made incorrectly. Instead of arriving at 793 by incorrect means earlier in the process we proceed carefully and correctly and work backwards from f(793) iteratively:

$$ f(

BOXED []
BOXED FINAL 
eval() arg 1 must be a string, bytes or code object final_eval
[(199, 2), (203, 2), (791, 2), (251, 1)]
code_answers 3 text_answers 4



## QUESTION 4 - 5 
- TIME_SPENT : 879 secs

5_User:

Below is a math problem you are to solve (positive numerical answer):
"A function $f: \mathbb N \to \mathbb N$ satisfies the following two conditions for all positive integers $n$:$f(f(f(n)))=8n-7$ and $f(2n)=2f(n)+1$. Calculate $f(100)$."
To accomplish this, first determine a sympy-based approach for solving the problem by listing each step to take and what functions need to be called in each step. Be clear so even an idiot can follow your instructions, and remember, your final answer should be positive integer, not an algebraic expression!
Write the entire script covering all the steps (use comments and document it well) and print the result. After solving the problem, output the final numerical answer within \boxed{}.

Assistant: 

Interesting, let's analyze step by step:



First, we know that `f(f(f(n))) = 8n - 7` and `f(2n) = 2f(n) + 1`.
Let's start by computing `f(1)` from the second equation. We plug `n = 1`, which gives us `f(2) = 2f(1) + 1`. Unfortunately, this equation alone is not sufficient to find the value of `f(1)`. We need to work with the first equation. By plugging in `n = 1`, we get `f(f(f(1))) = 8*1 - 7 = -1`. However, this information is not very useful without additional information. The function values are natural numbers, but we get a negative number. This leads us to think of a recursive approach, specifically one that attempts to find `f(1)` first and then use that to find the values of other function evaluations through the equations given.

Let's compute `f(1)` assuming `f` is defined on the natural numbers as a recursive function.

Let `g(k) = f^k(1)`, which stands for `f` iterated `k` times starting from 1. We note from `f(2n) = 2f(n) + 1` for `n = 1`:
\[g(2) = f(f(1)) = f(g(1)) = f(1) = 2f(1) + 1.\]
Plugging in `g(1)` on the left hand side and `f(1)` on the right we have:
\[2g(1) + 1 = 8*1 - 7 = -1.\]
However this can't be right, we expected positive integers and obtained a negative value. Let's try applying the first equation on `g(3)`:
\[8*1 - 7 = -1 \implies g(3) = -1 \implies f(g(2)) = -1 \implies f(f(1)) = -1.\]
Clearly something is not right, but we persisted so far just because it will lead somewhere (don't worry, we will fix this!).
Using the second function equation, we plug `n = g(1)`:
\[f(2g(1)) = 2f(g(1)) + 1 \implies f(2f(1)) = 2f(f(1)) + 1.\]
Now, replacing `f(f(1))` with `g(2)` we obtain:
\[f(2f(1)) = 2g(2) + 1.\]
On the right hand side, `2g(2) + 1` becomes:
\[2f(f(1)) + 1 = 2f(1) + 1 = 2*(-1) + 1 = -1.\]
Finally, with `f(2f(1)) = -1`, we apply the first function equation again, we plug `n = f(1)`:
\[f(f(f(1))) = 8*1 - 7 = -1 \implies g(3) = -1.\]
But this is exactly the expression we obtained before when we were applying `g(3) = -1`. This led to a contradiction as we initially knew natural numbers and ended up with -1. What went wrong?

As mentioned before, a negative value obtained does suggest a possible invalid manipulation or an inconsistent equation. To verify, let's retrace back our steps and make an observation. At one point, we ended up with the expression\[2f(1) + 1.\]But looking at the second function equation which contains `$f(2n) = 2f(n) + 1$`, the right hand side expression bears a very interesting similarity to our obtained expression except with `n` being `f(1)` which means we ended up with the right hand side part of the second function equation. The only way we can move forward at this point is to accept the inconsistency at the first two function equations we established, and hope a third function equation might help.

Luckily, we are not oblivious to other conditions provided earlier about the function, `f(f(f(n)) = 8n - 7`. Let's try computing for `f(1)` again but this time using the third equation. If we plug in `n = 1` the equation gives us:
\[f(f(f(1))) = f(f(1)) = 8*1 - 7 = 1 \implies f(1) = 1.\]
As $f$ is a function defined on the natural numbers, it seems reasonable that $f(1) = 1$, then we will just need to validate that indeed the other two equations agree with this value. Replacing `f(1)` by `1` in the two equations we stated initially:
\[f(2n) = 2f(n) + 1 = 2*1 + 1 = 3\] when `$n = 1$`. This satisfies the condition. For the second equation. When `n = f(1) = 1`, \[f(f(f(1))) = f(f(1)) = f(3) = 8*1 - 7 = 1.\]. Since, `f(3) = 1` and plugging this into the first equation:
\[f(f(f(3))) = f(f(1)) = f(3) = 1 = 8*3 - 7,\] holds. The values all agree with $f(1) = 1$ and thus we can confidently say that $f(1) = 1$. 
With this in mind and armed with the value of $f(1)$, we shall proceed with calculating \[f(100)= f^{3}(100).\] We just need to compute `f(f(f(100)))` which simplifies to`8 \cdot 100 - 7 = 793`. Therefore $f(100) = \boxed{793}.$ This will be the output of our computation:


```python


INTERMEDIATE OUT :

def f(n):
    return 8*n - 7

f_100 = f(f(f(100)))
print(f_100)
```

50689

CODE RESULTS 50689

INTERMEDIATE OUT :
```output
50689
```

This doesn't seem right. Let's look back at our functions. Something seems off with our mathematical approach. Let's try a different approach: since finding $f(1)$ through manipulation got us into a quagmire, let's try to use the actual function definition: if it takes three applications of the function to reach a known value, we should be able to calculate $f^{3}(n)$ for large $n$'s like 100 by repeatedly applying $f(n) = 8n - 7$. Unfortunately, we only have the value of $f(1) = 1$, and not a closed form for the function, and iterating the application of the function three times starting with 100 looks complex:  $f(f(f(100)))$ or more conveniently, $

BOXED ['793']
BOXED FINAL 793
[(199, 2), (203, 2), (791, 2), (251, 1), (689, 1), (793, 1)]
code_answers 4 text_answers 5



## QUESTION 4 - 6 
- TIME_SPENT : 879 secs

6_User:


Below is a math problem you are to solve (positive numerical answer!):
"A function $f: \mathbb N \to \mathbb N$ satisfies the following two conditions for all positive integers $n$:$f(f(f(n)))=8n-7$ and $f(2n)=2f(n)+1$. Calculate $f(100)$."
Analyze this problem and think step by step to come to a solution with programs. After solving the problem, output the final numerical answer within \boxed{}.

Assistant:

 To solve this problem, we can start by analyzing the two given conditions and see if we can find a pattern in the function $f$. 
Let's first try with $n=1$:
from the first condition, we get $f(f(f(1)))=8*1-7=1$,
which implies that $f(f(1))=1$.
Similarly, from the second condition with $n=1$, we have $f(2)=2f(1)+1$.
We are given that $f(f(f(1)))=1$, and $f(f(1))=1$ mean $f(1)$ is a fixed point of the function $f$.
Let's find another fixed point by setting $n=2$:
we have $f(f(f(2)))=8*2-7=9$,
which implies that $f(f(2))=9$.
Again, from the second condition with $n=2$, we have $f(4)=2f(2)+1$.
But we already know $f(f(2))=9$, so we can substitute $f(2)$ into the equation to get:
$f(4)=2(f(2))+1=2(2f(1)+1)+1=4f(1)+3$.
Now, substituting the value of $f(2)$, we can write: $9=4f(1)+3$. This implies that $4f(1)=6$ or $f(1)=1.5$, which contradicts our earlier finding that $f(1)$ is an integer.
However, we know that $f(1)$ is an integer. This leads us to a conclusion that there might be an error in our calculation. Let's retrace our steps and see what we did wrong.
It was a mistake to set $f(2)=2f(1)+1$. Notice that this would imply that $f(n)$ increases linearly as $n$ increases. But if $f(n)$ were to increase linearly, it wouldn't be possible for there to be a fixed point for $f$ (i.e., a value $a$ such that $f(a)=a$) because a linear function with a slope greater than 1 (such as the one implied by $f(n)=2f(n-1)+1$) will never map an input to itself.
Thus, it might be more helpful to try some other values to find a pattern in $f$. 
To gain some more insights, let's return to the original function equation $f(f(f(n)))=8n-7$. 
Setting $n=3$ gives:
$f(f(f(3)))=8*3-7=17$, so $f(f(3))=17$.
If we then apply the second condition for $n=3$, we find $f(6)=2f(3)+1=2(2f(1)+1)+1=4f(1)+3$. But we already found that $9=4f(1)+3$, so we must have $f(6)=9$. That means $f(3)=\frac{9}{2}$ - a non-integer. Uh oh, another mistake! Let's try a different approach.
Returning to the original function equation, we can set $n=1$ to find that $f(f(1))=1$. Let's set $f(1)=a$, then we get $f(a)=1$. 
Going back to the condition $f(f(f(n)))=8n-7$, with $n=a$, we have $f(f(a))=8a-7=1$, meaning that $8a=8$, so $a=1$.
That means $f(1)=1$. Now the condition $f(f(f(n)))=8n-7$ simply reduces to $f(f(n))=8n-8$.
Then with $n=1$ again, we get $f(f(1))=f(1)=8*1-8=0$, implying $f(1)=0$. Now our problem is that we have conflicting values for $f(1)$.
So we are going the wrong way - back to the drawing board.
If we take a step back, we realize that our mistake came from considering the function $f$ to be linear and trying to find an integer value for $f(1)$. We actually don't have to consider $f(1)$, we can just jump right into considering the function $f$ that satisfies $f(f(f(n)))=8n-7$. We know from the first part of the problem that one possible function that satisfies this condition is the function $f(n)=2n-1$, we can check this by substitution.
Now with $f(n)=2n-1$, we indeed get $f(f(f(n)))=(2(2n-1)-1)=4n-3=8n-7$. To show that this indeed is the function $f$, we can now use mathematical induction to show that $f(n)=2n-1$ for all positive integers $n$.
Base case: We showed above that $f(1)=1=2*1-1$.
Inductive step: Assume that $f(k)=2k-1$ holds for some positive integer $k$. We will show that $f(k+1)=2(k+1)-1$.
Since $f(k)=2k-1$, we apply the second condition to find that $f(2k)=2f(k)+1=2(2k-1)+1=4k-1$, and thus $f(f(k))=f(2k-1)=4k-3$.
Then applying $f(f(f(k)))=8k-7$, we get $f(4k-3)=8k-7$, and that means $f(k+1)=2(k+1)-1$. By the principle of mathematical induction, $f(n)=2n-1$ for all positive integers $n$.
Finally, we are asked to find the value of $f(100)$. We simply plug in $n=100$ into $f(n)=2n-1$, to get $f(100)=2*100-1=199$. So the value of $f(100)$ is $199$. So to return to our original question of solving this problem programmatically, we could just define the function $f(n)=2n-1$ and then plug in $n=100$ to find $f(100)$:

```python


INTERMEDIATE OUT :

def f(n):
    return 2*n - 1

f_100 = f(100)
print(f_100)
```

199

CODE RESULTS 199

INTERMEDIATE OUT :
```output
199
```
The value of $f(100)$ is $\boxed{199}$. Note that in this specific problem, you can arrive at the answer more easily without programming if you realize that the function $f(n)=2n-1$ is the only function that satisfies the conditions $f(f(f(n)))=8n-7$

BOXED ['199']
BOXED FINAL 199
[(199, 4), (203, 2), (791, 2), (251, 1), (689, 1), (793, 1)]
GOOD ANSWER UPDATED!
ANSWER FOUND!
Predicted best answer: {0: (112, 2), 1: (800, 3), 2: (199, 3), 3: (256, 4), 4: (199, 4)}

prompt correctness:[1, 1]

## Self-Reflections

### Question 4 0 reflection:
None
### Question 4 1 reflection:
None
### Question 4 2 reflection:
None
### Question 4 3 reflection:
None
### Question 4 4 reflection:
None
### Question 4 5 reflection:
None
### Question 4 6 reflection:
None
---
