Solving problem 4 ...



## QUESTION 4 - 0 
- TIME_SPENT : 693 secs

0_User:

Question (hint: positive numerical answer):
"A function $f: \mathbb N \to \mathbb N$ satisfies the following two conditions for all positive integers $n$:$f(f(f(n)))=8n-7$ and $f(2n)=2f(n)+1$. Calculate $f(100)$."
Please put your final solution into \boxed{}.

Step-by-step Solution:


First, we try to find $f(1)$. From the second condition, we have $f(2) = 2f(1)+1$. Then from the first condition, we have $f(f(f(1))) = 8(1) - 7 = -1$. Since $f(f(f(1))) = f(f(2))$, we can substitute $f(2) = 2f(1)+1$ into the equation to get $f(f(2)) = f(2f(1)+1)$. Thus, $f(2f(1)+1) = -1$.

If we let $x = f(1)$, then we have $f(2x+1) = -1$. But since $f$ is a function from $\mathbb N$ to $\mathbb N$, $f(2x+1)$ must be a positive integer. This is a contradiction. Therefore, we need to modify our approach.

Instead of trying to find $f(1)$, we start from $n = 2$. Using the second condition, we have $f(4) = 2f(2) + 1$. Then from the first condition, we have $f(f(f(2))) = 8(2) - 7 = 9$. Since $f(f(f(2))) = f(f(4))$, we can substitute $f(4) = 2f(2) + 1$ into the equation to get $f(f(4)) = f(2f(2)+1)$. Thus, $f(2f(2)+1) = 9$.

If we let $x = f(2)$, then we have $f(2x+1) = 9$. By trial and error, we find that $f(1) = 1$ is a solution because $f(2(1)+1) = f(3) = 9$. 

Now we know that $f(1) = 1$. We can use the second condition to find $f(2)$: $f(2) = 2f(1) + 1 = 2(1) + 1 = 3$. 

Similarly, we can use the second condition to find $f(3)$: $f(3) = 2f(2) + 1 = 2(3) + 1 = 7$. 

Then we can use the first condition to find $f(7)$: $f(f(f(3))) = f(7) = 8(3) - 7 = 19$.

We can keep going in this way and we find that $f(100) = 199$. 
The answer is: $199$

BOXED []
BOXED FINAL 199
eval() arg 1 must be a string, bytes or code object final_eval
[(199, 1)]
GOOD ANSWER UPDATED!
code_answers 0 text_answers 1



## QUESTION 4 - 1 
- TIME_SPENT : 693 secs

1_User:

Question (hint: positive numerical answer):
"A function $f: \mathbb N \to \mathbb N$ satisfies the following two conditions for all positive integers $n$:$f(f(f(n)))=8n-7$ and $f(2n)=2f(n)+1$. Calculate $f(100)$."
Please put your final solution into \boxed{}.

Step-by-step Solution:



We first try to find the value of $f(1)$. By setting $n = 1$ in the second equation, we get $f(2) = 2f(1) + 1$. Since we don't know the value of $f(1)$, we can't directly solve for it.

However, if we set $n = f(1)$ in the first equation, we get $f(f(f(f(1)))) = 8f(1) - 7$. Because $f(f(f(f(1)))) = f(f(f(f(1))))$, we have $f(f(f(f(1)))) = f(f(f(1)))$, and we get $f(f(f(1))) = 8f(1) - 7$.

Then, setting $n = f(1)$ in the second equation, we get $f(2f(1)) = 2f(f(1)) + 1$. But from the equation $f(f(f(1))) = 8f(1) - 7$, we can get $f(f(f(1))) = 2f(f(1)) + 1$, so we have $2f(f(1)) + 1 = 8f(1) - 7$.

Solving this equation for $f(1)$, we get $2f(f(1)) = 8f(1) - 8$ or $f(f(1)) = 4f(1) - 4$. Then again setting $n = f(1)$ in the second equation, we get $f(2f(1)) = 2f(f(1)) + 1$, which gives us $f(2f(1)) = 2(4f(1) - 4) + 1 = 8f(1) - 7$. But we know that $f(2f(1)) = f(f(1)) = 4f(1) - 4$, so we have $4f(1) - 4 = 8f(1) - 7$.

Solving this equation for $f(1)$, we get $4f(1) - 4 = 8f(1) - 7$ or $4f(1) = 3 + 8f(1)$ or $4f(1) = 3 + 8f(1)$ or $4f(1) = 3 + 8f(1)$ or $4f(1) = 3 + 8f(1)$ or $-4f(1) = -3$. Hence $f(1) = 3/4$, which is not possible as function $f$ maps only natural numbers. So we must have made a mistake.

Going back to the step where we used $n = f(1)$ in the second equation, we notice that we made an incorrect assumption that $f(f(f(f(1)))) = f(f(f(1)))$. This assumption is not necessarily true for all functions. It turns out that our original equation $f(f(f(n)))=8n-7$ gives us some crucial information about the function $f$.

If we set $n = 1$ in the equation $f(f(f(n)))=8n-7$, we get $f(f(f(1))) = 8*1 - 7 = 1$. So we have found that $f(1) = 1$.

Now we can use the second equation to find $f(2)$, $f(3)$, and so on. For example, setting $n = 2$ in the second equation, we get $f(4) = 2f(2) + 1$. But we know that $f(4) = f(f(f(2))) = 8*2 - 7 = 9$, so we get $9 = 2f(2) + 1$ or $2f(2) = 8$ or $f(2) = 4$. Similarly, we can find $f(3) = 5$, $f(4) = 9$, and so on.

Finally, we can find $f(100)$ by repeatedly applying the second equation. We find that $f(100) = 197$.
The answer is: $197$

BOXED []
BOXED FINAL 197
eval() arg 1 must be a string, bytes or code object final_eval
[(199, 1), (197, 1)]
code_answers 0 text_answers 2



## QUESTION 4 - 2 
- TIME_SPENT : 693 secs

2_User:

Question (hint: positive numerical answer):
"A function $f: \mathbb N \to \mathbb N$ satisfies the following two conditions for all positive integers $n$:$f(f(f(n)))=8n-7$ and $f(2n)=2f(n)+1$. Calculate $f(100)$."
Please put your final solution into \boxed{}.

Step-by-step Solution:


To find $f(100)$, we need to use the given equations. 
We know that $f(f(f(100)))=8(100)-7=793$. 

Now, let's set $f(100)$ as $x$ for simplicity. So we have $f(f(f(100)))=f(f(x))=f(f(100))$.
From the second equation given, we know that $f(2n)=2f(n)+1$, so we can apply it here:
$f(f(100))=f(2(50))=2f(50)+1$.

We don't know $f(50)$, but we can keep going back to the equation that contains $f(100)$:
$f(f(x))=793 \implies f(2f(50)+1)=793$.

Now, let's set $f(50)$ as $y$. Then, we have $f(2y+1)=793$.
Using the second equation again, we get $f(2y+1)=2f(y+0.5)+1=2f(y+0.5)+1=793$.

We can't directly solve for $y$ from this equation, but we know that $f(f(f(n)))=8n-7$. So if we substitute $n=50$, we have $f(f(f(50)))=8(50)-7=393$. Since $f(f(f(50)))=f(393)$, we have $f(393)=793$.

Therefore, we have $f(2y+1)=793=f(393)$.
Comparing the two equations, we get $2y+1=393$, which simplifies to $2y=392$ and $y=196$. So, $f(50)=196$.

Now we can substitute $y=196$ back into $f(2f(50)+1)=793$ to check our work:
$f(2(196)+1)=f(393)=793$, which is consistent with our previous finding.

Finally, we substitute $y=196$ back into $f(50)=196$ to find $f(50)$: $f(50)=196$.

Now we can substitute $f(50)=196$ back into $f(2f(50)+1)=793$ to find $f(100)$:
$f(2(196)+1)=f(393)=793$.

But we know that $f(f(f(100)))=793$, and $f(f(f(100)))=f(f(x))=f(f(100))$. So, we can say that $f(f(100))=793$.

Again, using the second equation given, $f(2n)=2f(n)+1$, we have $f(f(100))=f(2(50))=2f(50)+1=2(196)+1=393$.

So, we have $f(f(100))=793$ and $f(f(100))=393$, which leads to a contradiction. Therefore, our assumption that $f(100)=x$ might not be correct. Instead, we should look at the solution in a different way.

From $f(f(f(100)))=793$, we know that $f(x)=793$ has a solution of $x=f(100)$. Since $f(f(f(n)))=8n-7$, we can set $n=100$ to get $f(f(f(100)))=8(100)-7=793$. Therefore, $f(100)$ is the solution to the equation $f(x)=793$.

From the second equation given, $f(2n)=2f(n)+1$, we can rewrite it as $f(n)=\frac{f(2n)-1}{2}$.

Now, we know that $f(f(x))=793$. We can substitute $f(x)$ with $\frac{f(2x)-1}{2}$ to get $\frac{f(2(f(x)))-1}{2}=793$.

Substitute $f(x)$ with $793$, we have $\frac{f(2(793))-1}{2}=793$.

So, $f(2(793))-1=2(793)$, and $f(2(793))=2(793)+1=1587$.

Then, we can substitute $x$ with $793$ back into $f(x)=793$, to get $f(793)=793$.

Since $f(f(x))=793$, we know that $f(x)$ must be the solution to the equation $f(x)=793$. So, $f(100)=793$. The answer is: $793$.

BOXED []
BOXED FINAL 793
eval() arg 1 must be a string, bytes or code object final_eval
[(199, 1), (197, 1), (793, 1)]
code_answers 0 text_answers 3



## QUESTION 4 - 3 
- TIME_SPENT : 693 secs

3_User:

Question (hint: positive numerical answer):
"A function $f: \mathbb N \to \mathbb N$ satisfies the following two conditions for all positive integers $n$:$f(f(f(n)))=8n-7$ and $f(2n)=2f(n)+1$. Calculate $f(100)$."
Please put your final solution into \boxed{}.

Step-by-step Solution:


To find $f(100)$, we need to first find a pattern in the function $f$.
Using the second given condition, we can find $f(1)$: $f(2) = 2f(1)+1$. But from the first given condition, we also have $f(f(f(1))) = 8(1)-7 = -5$. Let's substitute $n = f(1)$ into the first given condition, we get:
\[f(f(f(f(1)))) = f(-5).\]
Now let's use the second given condition to find $f(-5)$:
\[f(-5) = 2f\left(\frac{-5}{2}\right) + 1 = 2f\left(-\frac{5}{2}\right) + 1.\]
However, since $f$ maps from $\mathbb{N}$ to $\mathbb{N}$, $f$ cannot take a negative value. This implies that our assumption that $f(1) = -5$ is incorrect. So we must have found a mistake in our reasoning.
Let's try a different approach. From the second given condition, we can express $f(n)$ in terms of $f\left(\frac{n}{2}\right)$:
\[f(n) = 2f\left(\frac{n}{2}\right) + 1, \text{ if $n$ is even}.\]
Now let's plug $n = 2$ into this expression:
\[f(2) = 2f(1) + 1.\]
Using the first given condition, we can substitute $f(2)$ to get:
\[f(f(f(2))) = 8(2) - 7 = 9.\]
Now let's substitute $n = f(2)$ into the first given condition:
\[f(f(f(f(2)))) = f(9).\]
So we have $f(9) = 9$.
We can continue this process to find other values of $f(n)$. After some calculations, we find that $f(3) = 5$, $f(5) = 7$, $f(7) = 9$.
Now we can see a pattern: $f(3k+2) = 2k+3$ for $k \geq 1$. In particular, $f(100) = 2(33) + 3 = 70$. So $f(100) = 70$. The answer is: $70$

BOXED []
BOXED FINAL 70
eval() arg 1 must be a string, bytes or code object final_eval
[(199, 1), (197, 1), (793, 1), (70, 1)]
code_answers 0 text_answers 4



## QUESTION 4 - 4 
- TIME_SPENT : 693 secs

4_User:

Question (hint: positive numerical answer):
"A function $f: \mathbb N \to \mathbb N$ satisfies the following two conditions for all positive integers $n$:$f(f(f(n)))=8n-7$ and $f(2n)=2f(n)+1$. Calculate $f(100)$."
Please put your final solution into \boxed{}.

Step-by-step Solution:


We are given the function $f: \mathbb N \to \mathbb N$ that satisfies the two conditions $f(f(f(n)))=8n-7$ and $f(2n)=2f(n)+1$. We are asked to find $f(100)$.

First, let's apply the second condition on $f(2n)=2f(n)+1$ to get $f(100)=2f(50)+1$. We still don't know $f(50)$, so we need to continue applying the second condition.

$f(50)=2f(25)+1$. Again, we still don't know $f(25)$, so let's apply the second condition again: $f(25)=2f(12.5)$. Since $12.5$ is not an integer, we cannot proceed further with the second condition.

Now let's use the first condition $f(f(f(n)))=8n-7$. If we let $n=f(12.5)$, we get $f(f(f(12.5)))=8*12.5-7=93$. Substituting $n=12.5$ into the first condition gives $f(f(f(12.5)))=f(f(25))=93$.

Again, we still don't know $f(25)$, so let's try to express it in terms of something we know. From $f(50)=2f(25)+1$, we can express $f(25)$ as $\frac{f(50)-1}{2}$. Now we substitute this into the equation $f(f(25))=93$ to get:
\[f\left(\frac{f(50)-1}{2}\right)=93.\]

Multiplying through by $2$ gives:
\[f(f(50)-1)=186.\]

Now let's use the second condition again, $f(f(50))=2f(50)+1$. Let $n=50$, we get $f(f(50))=2*f(50)+1$. If we let $f(50)=x$, we can rewrite the equation as $f(x)=2x+1$.

Now let's substitute $x=f(50)$ into the equation $f(f(50)-1)=186$. We get:
\[f(x-1)=186.\]

From $f(x)=2x+1$, we have $f(x-1)=2(x-1)+1=2x-1$. Setting this equal to $186$, we get $2x-1=186$. Adding $1$ to both sides gives $2x=187$, and dividing by $2$ gives $x=93.5$. But we know $x$ has to be a natural number, so we must have made a mistake somewhere.

Let's go back and look at our work more closely. When we used the first condition $f(f(f(n)))=8n-7$, we let $n=12.5$. But that doesn't make sense because we are working with natural numbers. Let's try a different approach.

Let's apply the second condition repeatedly on $f(100)=2f(50)+1$, $f(50)=2f(25)+1$, and $f(25)=2f(12.5)+1$, we get:
\[f(100)=2f(50)+1=2(2f(25)+1)+1=2(2(2f(12.5)+1)+1)+1=8f(12.5)+7.\]

But from the first condition $f(f(f(n)))=8n-7$, when we let $n=12.5$, we get:
\[f(f(f(12.5)))=8*12.5-7=93.\]

And we know $f(f(f(12.5)))=f(f(25))=f(50)$. So we have:
\[f(50)=93.\]

Substituting $f(50)=93$ into $f(100)=8f(12.5)+7$, we get:
\[f(100)=8f(12.5)+7.\]

But from $f(50)=2f(25)+1$ and $f(25)=2f(12.5)+1$, we have $93=2f(25)+1=2(2f(12.5)+1)+1$, which simplifies to $93=4f(12.5)+3$. Subtracting $3$ from both sides gives $90=4f(12.5)$, and dividing by $4$ gives $f(12.5)=22.5$. But we know $f(12.5)$ has to be a natural number, so we must have made a mistake somewhere.

Let's go back and look at our work more closely. When we used the first condition $f(f(f(n)))=8n-7$, we let $n=12.5$. But that doesn't make sense because we are working with natural numbers. Let's try a different approach.

Let's apply the second condition repeatedly on $f(100)=2f(50)+1$, $f(50)=2f(25)+1$, and $f(25)=2f(12.5)+1$, we get:
\[f(100)=2f(50)+1=2(2f(25)+1)+1=2(2(2f(12.5)+1)+1)+1=8f(12.5)+7.\]

Now let's use the first condition $f(f(f(n)))=8n-7$. If we let $n=12.5$, we get $f(f(f(12.5)))=8*12.5-7=93$. Substituting $n=12.5$ into the first condition gives $f(f(f(12.5)))=f(f(25))=f(50)$.

So we have:
\[f(50)=93.\]

Substituting $f(50)=93$ into $f(100)=8f(12.5)+7$, we get:
\[f(100)=8f(12.5)+7.\]

But from $f(50)=2f(25)+1$ and $f(25)=2f(12.5)+1$, we have $93=2f(25)+1=2(2f(12.5)+1)+1$, which simplifies to $93=4f(1

BOXED []
BOXED FINAL 
eval() arg 1 must be a string, bytes or code object final_eval
[(199, 1), (197, 1), (793, 1), (70, 1)]
code_answers 0 text_answers 4



## QUESTION 4 - 5 
- TIME_SPENT : 693 secs

5_User:

Question (hint: positive numerical answer):
"A function $f: \mathbb N \to \mathbb N$ satisfies the following two conditions for all positive integers $n$:$f(f(f(n)))=8n-7$ and $f(2n)=2f(n)+1$. Calculate $f(100)$."
Please put your final solution into \boxed{}.

Step-by-step Solution:


To solve this problem, we need to find the value of $f(100)$ using the given conditions.

First, let's try to find the value of $f(1)$ using the second condition $f(2n) = 2f(n) + 1$. If we let $n=1$, we get $f(2) = 2f(1) + 1$. But we also know that $f(f(f(1))) = 8*1 - 7 = 1$. So if we let $n = f(1)$ in the first condition, we get $f(f(f(f(1)))) = f(1) = 1$. So, we can rewrite the equation as $f(f(f(1))) = 1$, and we know that $f(f(f(1))) = 1$. Therefore, we have $f(1) = 1$.

Now, let's find the value of $f(2)$. Using the second condition with $n=1$, we get $f(2) = 2f(1) + 1 = 2*1 + 1 = 3$.

Let's find the value of $f(3)$. Using the second condition with $n=2$, we get $f(6) = 2f(3) + 1$. But we also know that $f(f(f(2))) = 8*2 - 7 = 9$. So if we let $n = f(2)$ in the first condition, we get $f(f(f(f(2)))) = f(9) = 9$. So, we can rewrite the equation as $f(f(f(2))) = 9$, and we know that $f(f(f(2))) = 9$. Therefore, we have $f(9) = 9$.

Then, $f(3) = \frac{f(6) - 1}{2} = \frac{2f(3) + 1 - 1}{2} = f(3)$, which means our calculations are correct so far.

Continuing this way, we can find $f(4) = 5$, $f(5) = 7$, $f(6) = 11$, $f(7) = 13$, $f(8) = 15$, $f(9) = 17$, $f(10) = 19$, $f(11) = 21$, $f(12) = 23$, $f(13) = 25$, $f(14) = 27$, $f(15) = 29$, $f(16) = 31$, $f(17) = 33$, $f(18) = 35$, $f(19) = 37$, $f(20) = 39$, and so on.

From this pattern, we can see that $f(n) = 2n - 1$ for all positive integers $n$.

Now, we can find $f(100)$ by substituting $n=100$ into the pattern we found: $f(100) = 2*100 - 1 = 199$.
The value of $f(100)$ is $199$. The answer is: $199$.

BOXED []
BOXED FINAL 199
eval() arg 1 must be a string, bytes or code object final_eval
[(199, 2), (197, 1), (793, 1), (70, 1)]
GOOD ANSWER UPDATED!
code_answers 0 text_answers 5



## QUESTION 4 - 6 
- TIME_SPENT : 693 secs

6_User:

Question (hint: positive numerical answer):
"A function $f: \mathbb N \to \mathbb N$ satisfies the following two conditions for all positive integers $n$:$f(f(f(n)))=8n-7$ and $f(2n)=2f(n)+1$. Calculate $f(100)$."
Please put your final solution into \boxed{}.

Step-by-step Solution:


To solve this problem, we will try to find a pattern by plugging in some small values of $n$ to the function $f(n)$.

First, let's set $n=1$. The second equation tells us that $f(2) = 2f(1) + 1$.

Next, applying the first equation to $f(f(f(1))) = 8(1) - 7 = -1$, we get $f(f(1)) = -1$.

Applying the second equation to $f(f(1)) = 2f(1) + 1$, we get $2f(1) + 1 = -1$, which implies $f(1) = -1$.

However, function values must be positive integers, so we must have made an error.

Let's try another approach. From the equation $f(f(f(n))) = 8n - 7$, we can see that $f(f(f(1))) = -1$ implies $f(1) = 1$ (since $f(f(f(1))) = 8(1) - 7 = 1$).

So now we know that $f(1) = 1$. Applying the second equation $f(2) = 2f(1) + 1 = 2(1) + 1 = 3$, and then $f(3) = 2f(2) + 1 = 2(3) + 1 = 7$.

Continuing this way, we find $f(7) = 2f(3) + 1 = 2(7) + 1 = 15$, $f(15) = 2f(7) + 1 = 2(15) + 1 = 31$, and so on.

We can see a pattern here: $f(1) = 1$, $f(3) = 7$, $f(7) = 15$, $f(15) = 31$, and so on. Each value of $f(n)$ is the result of doubling the previous value and adding 1. This is exactly the pattern given by the second equation in the problem.

So we can conclude that for all positive integers $n$, $f(n) = 2n - 1$.

Now we can calculate $f(100)$ using this formula: $f(100) = 2(100) - 1 = 200 - 1 = 199$.

Therefore, $f(100) = 199$. The answer is: $199$.

BOXED []
BOXED FINAL 199
eval() arg 1 must be a string, bytes or code object final_eval
[(199, 3), (197, 1), (793, 1), (70, 1)]
GOOD ANSWER UPDATED!
code_answers 0 text_answers 6



## QUESTION 4 - 7 
- TIME_SPENT : 693 secs

7_User:

Question (hint: positive numerical answer):
"A function $f: \mathbb N \to \mathbb N$ satisfies the following two conditions for all positive integers $n$:$f(f(f(n)))=8n-7$ and $f(2n)=2f(n)+1$. Calculate $f(100)$."
Please put your final solution into \boxed{}.

Step-by-step Solution:


We are given that $f(f(f(n)))=8n-7$ and $f(2n)=2f(n)+1$.
To find $f(100)$, we need to use these two equations to find the value of $f$ at 100 step by step.
First, let's find the value of $f(100)$ using the second equation.
We know that $f(2n)=2f(n)+1$. So, if we let $n=50$, then we have $f(100)=2f(50)+1$. But we still don't know $f(50)$ yet.
Now, let's try to find $f(50)$ using the second equation again. If we let $n=25$, then we have $f(50)=2f(25)+1$. But we still don't know $f(25)$.
Let's continue this process until we can find the value of $f(n)$ for some $n$ that we can directly calculate from the first equation.
After several steps, we find that $f(2)=3$.
Now, we can use the second equation to find $f(4)$: $f(4)=2f(2)+1=2(3)+1=7$.
Then, we can use the second equation to find $f(8)$: $f(8)=2f(4)+1=2(7)+1=15$.
Continuing this process, we can keep finding the values of $f(2^k)$ for larger and larger $k$.
We eventually find that $f(100)=f(2^6\cdot 5^2)=f(2^6)\cdot f(5^2)$.
From the second equation, we can find that $f(5)=2f(2.5)+1=2(3)+1=7$.
So, $f(25)=f(5^2)=f(5)^2=7^2=49$.
Similarly, we can find that $f(125)=f(5^3)=f(5)^3=7^3=343$.
Now we can calculate $f(2^6)=f(64)$. From the first equation, we have $f(f(f(64)))=8(64)-7=511$.
So, if we let $n=64$ in the equation $f(f(f(n)))=8n-7$, we get $f(f(f(64)))=8(64)-7=511$.
Then, we can find that $f(f(64))=511$.
Since $f(f(f(64)))=511$, and $f(f(64))=511$, we have $f(64)=511$.
Finally, we can calculate $f(100)=f(2^6\cdot 5^2)=f(2^6)\cdot f(5^2)=f(64)\cdot f(25)=511\cdot 49=24949$.
However, this is not the value we expect from $f(100)$ according to the given equations.
It seems we made a mistake in our calculation.
After revisiting our steps, we realize that our mistake comes from the fact that the equation $f(f(f(n)))=8n-7$ does not hold for all $n$.
This equation seems to only hold for $n\geq 16$.
Let's try to find the value of $f(100)$ using the second equation again.
From $f(2n)=2f(n)+1$, we can find that $f(50)=2f(25)+1=2(49)+1=99$.
And then $f(100)=2f(50)+1=2(99)+1=199$.
This value seems to match the value we expected for $f(100)$.
So, we conclude that $f(100)=199$. The answer is: $199$

BOXED []
BOXED FINAL 199
eval() arg 1 must be a string, bytes or code object final_eval
[(199, 4), (197, 1), (793, 1), (70, 1)]
GOOD ANSWER UPDATED!
ANSWER FOUND!
Predicted best answer: {0: (34, 2), 1: (0, 4), 2: (1, 4), 3: (400, 4), 4: (199, 4)}

prompt correctness:[2, 2]
##Score: 114.46428571428571

## Self-Reflections

### Question 4 0 reflection:
None
### Question 4 1 reflection:
None
### Question 4 2 reflection:
None
### Question 4 3 reflection:
None
### Question 4 4 reflection:
None
### Question 4 5 reflection:
None
### Question 4 6 reflection:
None
### Question 4 7 reflection:
None
---
