Solving problem 0 ...



## QUESTION 0 - 0 
- TIME_SPENT : 0 secs

0_User:

Below is a math problem you are to solve (positive numerical answer!):
"Let $k, l > 0$ be parameters. The parabola $y = kx^2 - 2kx + l$ intersects the line $y = 4$ at two points $A$ and $B$. These points are distance 6 apart. What is the sum of the squares of the distances from $A$ and $B$ to the origin?"
Analyze this problem and think step by step to come to a solution with programs. After solving the problem, output the final numerical answer within \boxed{}.

Assistant:

 To solve this problem, we first need to find the coordinates of points $A$ and $B$.

The parabola $y = kx^2 - 2kx + l$ intersects the line $y = 4$ when $kx^2 - 2kx + l = 4$. This simplifies to $kx^2 - 2kx + l - 4 = 0$. Let's call this equation (1).

The distance between points $A$ and $B$ is given as 6. The distance formula in terms of coordinates is $\sqrt{(x_2 - x_1)^2 + (y_2 - y_1)^2}$. Here, $y_1 = y_2 = 4$, so the distance formula simplifies to $|x_2 - x_1| = 6$. Since the roots of equation (1) are the x-coordinates of $A$ and $B$, we can write this as $|x_2 - x_1| = 6 \Rightarrow x_2 - x_1 = 6$ or $x_2 - x_1 = -6$. Let's call these equations (2) and (3), respectively.

Now, let's find the sum of the squares of the distances from $A$ and $B$ to the origin. The distance from a point $(x, y)$ to the origin $(0, 0)$ is $\sqrt{x^2 + y^2}$. For points $A$ and $B$, this is $\sqrt{x_1^2 + 4^2}$ and $\sqrt{x_2^2 + 4^2}$, respectively. So, the sum of the squares of the distances is $x_1^2 + 16 + x_2^2 + 16 = x_1^2 + x_2^2 + 32$.

We know that the sum of the roots of equation (1) is given by $\frac{2k}{k} = 2$, and the product of the roots is given by $\frac{l - 4}{k}$. From equation (2), we have $x_2 - x_1 = 6$, which can be rewritten as $x_2 = x_1 + 6$. Squaring both sides gives $x_2^2 = x_1^2 + 12x_1 + 36$. Substituting this into the sum of squares of distances gives $x_1^2 + (x_1 + 6)^2 + 32 = x_1^2 + x_1^2 + 12x_1 + 36 + 32 = 2x_1^2 + 12x_1 + 68$.

We also know that $x_1$ and $x_2$ are the roots of equation (1), so by Vieta's formulas, $x_1 + x_2 = 2$ and $x_1x_2 = \frac{l - 4}{k}$. From equation (2), we have $x_2 = x_1 + 6$, so substituting this into the sum of roots equation gives $x_1 + (x_1 + 6) = 2 \Rightarrow 2x_1 + 6 = 2 \Rightarrow 2x_1 = -4 \Rightarrow x_1 = -2$. Substituting $x_1 = -2$ into the product of roots equation gives $(-2)((-2) + 6) = \frac{l - 4}{k} \Rightarrow 8 = \frac{l - 4}{k} \Rightarrow l - 4 = 8k \Rightarrow l = 8k + 4$.

Substituting $x_1 = -2$ into the sum of squares of distances equation gives $2(-2)^2 + 12(-2) + 68 = 8 - 24 + 68 = 52$. So, the sum of the squares of the distances from $A$ and $B$ to the origin is 52. The answer is: $52$

BOXED []
BOXED FINAL 52
eval() arg 1 must be a string, bytes or code object final_eval
[(52, 1)]
GOOD ANSWER UPDATED!
code_answers 0 text_answers 1



## QUESTION 0 - 1 
- TIME_SPENT : 0 secs

1_User:

Below is a math problem you are to solve (positive numerical answer!):
"Let $k, l > 0$ be parameters. The parabola $y = kx^2 - 2kx + l$ intersects the line $y = 4$ at two points $A$ and $B$. These points are distance 6 apart. What is the sum of the squares of the distances from $A$ and $B$ to the origin?"
Analyze this problem and think step by step to come to a solution with programs. After solving the problem, output the final numerical answer within \boxed{}.

Assistant:

 To solve this problem, we first need to find the x-coordinates of points A and B, then calculate the distances from A and B to the origin, and finally square these distances and sum them up.

Let's start by finding the x-coordinates of points A and B. The parabola $y = kx^2 - 2kx + l$ intersects the line $y = 4$, so we have:
$$4 = kx^2 - 2kx + l.$$
Rearranging the equation gives:
$$kx^2 - 2kx + l - 4 = 0.$$
This is a quadratic equation in x. Since the parabola intersects the line at two points A and B, the quadratic equation has two distinct roots, say $x_1$ and $x_2$, which are the x-coordinates of A and B. We are given that the distance between A and B is 6, so we have $|x_2 - x_1| = 6$.

Now, let's calculate the distances from A and B to the origin. The distance from a point $(x, y)$ to the origin is $\sqrt{x^2 + y^2}$. For point A with coordinates $(x_1, 4)$, the distance to the origin is $\sqrt{x_1^2 + 4^2} = \sqrt{x_1^2 + 16}$. Similarly, for point B with coordinates $(x_2, 4)$, the distance to the origin is $\sqrt{x_2^2 + 16}$.

Next, we square these distances: $(x_1^2 + 16)$ and $(x_2^2 + 16)$. We are asked to find the sum of the squares of the distances, so we need to calculate $(x_1^2 + 16) + (x_2^2 + 16) = x_1^2 + x_2^2 + 32$.

Finally, we need to find the value of $x_1^2 + x_2^2$ using the fact that $|x_2 - x_1| = 6$. The sum of the squares of the roots of a quadratic equation $ax^2 + bx + c = 0$ is given by $\frac{b^2 - 2ac}{a^2}$. In our case, $a = k$, $b = -2k$, and $c = l - 4$. So we have:
$$x_1^2 + x_2^2 = \frac{(-2k)^2 - 2k(l - 4)}{k^2} = \frac{4k^2 - 2kl + 8k}{k^2} = 4 - 2\frac{l}{k} + \frac{8}{k}.$$

Substituting this into our expression for the sum of the squares of the distances, we get:
$$4 - 2\frac{l}{k} + \frac{8}{k} + 32 = 36 - 2\frac{l}{k} + \frac{8}{k}.$$

However, we are not given enough information to determine the values of $k$ and $l$. Therefore, we cannot find the exact numerical value of the sum of the squares of the distances from A and B to the origin.

However, we have derived an expression for this sum in terms of $k$ and $l$:
$$36 - 2\frac{l}{k} + \frac{8}{k}.$$

If we are given the values of $k$ and $l$, we can substitute them into this expression to find the numerical value of the sum of the squares of the distances from A and B to the origin.
The answer is: $36 - 2\frac{l}{k} + \frac{8}{k}$.

BOXED []
BOXED FINAL 
eval() arg 1 must be a string, bytes or code object final_eval
[(52, 1)]
code_answers 0 text_answers 1



## QUESTION 0 - 2 
- TIME_SPENT : 0 secs

2_User:

Below is a math problem you are to solve (positive numerical answer!):
"Let $k, l > 0$ be parameters. The parabola $y = kx^2 - 2kx + l$ intersects the line $y = 4$ at two points $A$ and $B$. These points are distance 6 apart. What is the sum of the squares of the distances from $A$ and $B$ to the origin?"
Analyze this problem and think step by step to come to a solution with programs. After solving the problem, output the final numerical answer within \boxed{}.

Assistant:

 To solve this problem, we first need to find the $x$-coordinates of points $A$ and $B$. Since the parabola $y = kx^2 - 2kx + l$ intersects the line $y = 4$, we can set $kx^2 - 2kx + l = 4$. Rearranging the equation gives $kx^2 - 2kx + l - 4 = 0$. Let's call this equation (1).

We are given that the distance between points $A$ and $B$ is 6. Let $x_1$ and $x_2$ be the $x$-coordinates of $A$ and $B$ respectively. Then $x_2 - x_1 = 6$ or $x_1 - x_2 = 6$. By Vieta's formulas, we know that $x_1 + x_2 = \frac{2k}{k}$ and $x_1x_2 = \frac{l - 4}{k}$.

We can use these formulas to solve for $k$ and $l$. From $x_1 + x_2 = \frac{2k}{k}$, we get $2 = \frac{2k}{k}$, so $k = 1$. Then from $x_1x_2 = \frac{l - 4}{k}$, we get $x_1x_2 = l - 4$. Since $x_2 - x_1 = 6$, we can use the difference of squares to get $(x_2 - x_1)(x_2 + x_1) = 6(2)$, which simplifies to $x_1x_2 = 6$. Therefore, $l - 4 = 6$, so $l = 10$.

Now we have the parabola $y = x^2 - 2x + 10$. The points $A$ and $B$ are the solutions to the equation $x^2 - 2x + 10 = 4$, or $x^2 - 2x + 6 = 0$. Using the quadratic formula, we find that $x = 1 \pm i\sqrt{5}$. But the problem statement specifies that $k, l > 0$, so we must take the real parts of the solutions, which are $x = 1 \pm \sqrt{5}$. Let's call these $x_1$ and $x_2$.

The distances from $A$ and $B$ to the origin are $\sqrt{x_1^2 + y_1^2}$ and $\sqrt{x_2^2 + y_2^2}$, where $y_1 = 4$ and $y_2 = 4$. Therefore, the sum of the squares of the distances is
\[(\sqrt{x_1^2 + y_1^2})^2 + (\sqrt{x_2^2 + y_2^2})^2 = (x_1^2 + y_1^2) + (x_2^2 + y_2^2).\]
Substituting $y_1 = y_2 = 4$, we get
\[(x_1^2 + 16) + (x_2^2 + 16) = x_1^2 + x_2^2 + 32.\]
We know that $x_1^2 + x_2^2 = (x_1 + x_2)^2 - 2x_1x_2 = 2^2 - 2 \cdot 6 = 4 - 12 = -8$.

However, we made a mistake in our calculations. We should not have taken the real parts of the solutions to the equation $x^2 - 2x + 6 = 0$. Instead, we should have noted that the solutions to this equation are $x = 1 \pm i\sqrt{5}$, and the problem statement specifies that $k, l > 0$, so the solutions must be complex conjugates. Therefore, the $x$-coordinates of $A$ and $B$ are $1 + i\sqrt{5}$ and $1 - i\sqrt{5}$, respectively. The distances from $A$ and $B$ to the origin are $\sqrt{(1 + i\sqrt{5})^2 + 4}$ and $\sqrt{(1 - i\sqrt{5})^2 + 4}$, which simplify to $\sqrt{6 + 4i\sqrt{5}}$ and $\sqrt{6 - 4i\sqrt{5}}$. Taking the squares of these distances and adding them gives
\[(\sqrt{6 + 4i\sqrt{5}})^2 + (\sqrt{6 - 4i\sqrt{5}})^2 = (6 + 4i\sqrt{5}) + (6 - 4i\sqrt{5}) = 12.\]
Therefore, the sum of the squares of the distances from $A$ and $B$ to the origin is 12. The answer is: $12$

BOXED []
BOXED FINAL 12
eval() arg 1 must be a string, bytes or code object final_eval
[(52, 1), (12, 1)]
code_answers 0 text_answers 2



## QUESTION 0 - 3 
- TIME_SPENT : 0 secs

3_User:

Below is a math problem you are to solve (positive numerical answer!):
"Let $k, l > 0$ be parameters. The parabola $y = kx^2 - 2kx + l$ intersects the line $y = 4$ at two points $A$ and $B$. These points are distance 6 apart. What is the sum of the squares of the distances from $A$ and $B$ to the origin?"
Analyze this problem and think step by step to come to a solution with programs. After solving the problem, output the final numerical answer within \boxed{}.

Assistant:

 To solve this problem, we first need to find the x-coordinates of points $A$ and $B$.
The parabola $y = kx^2 - 2kx + l$ intersects the line $y = 4$, so we have:
\[4 = kx^2 - 2kx + l.\]
Rearranging terms, we get:
\[kx^2 - 2kx + l - 4 = 0.\]
Let's call this equation (1).

We are given that the points $A$ and $B$ are distance 6 apart. Let's call the x-coordinates of $A$ and $B$ as $x_1$ and $x_2$, respectively. Then, we have:
\[|x_2 - x_1| = 6.\]
By the quadratic formula, the roots of equation (1) are given by:
\[x = \frac{2k \pm \sqrt{(2k)^2 - 4k(l - 4)}}{2k} = 1 \pm \sqrt{1 - \frac{l - 4}{k}}.\]
Therefore, we have:
\[x_1 = 1 - \sqrt{1 - \frac{l - 4}{k}},\]
\[x_2 = 1 + \sqrt{1 - \frac{l - 4}{k}}.\]

Now, we need to find the sum of the squares of the distances from $A$ and $B$ to the origin. The distance from a point $(x, y)$ to the origin is $\sqrt{x^2 + y^2}$. For point $A$, this is $\sqrt{x_1^2 + 4^2}$, and for point $B$, this is $\sqrt{x_2^2 + 4^2}$. Therefore, the sum of the squares of the distances is:
\[(\sqrt{x_1^2 + 4^2})^2 + (\sqrt{x_2^2 + 4^2})^2 = x_1^2 + 16 + x_2^2 + 16 = x_1^2 + x_2^2 + 32.\]

Substituting the expressions for $x_1$ and $x_2$, we get:
\[(1 - \sqrt{1 - \frac{l - 4}{k}})^2 + (1 + \sqrt{1 - \frac{l - 4}{k}})^2 + 32.\]

We can simplify this expression using the identity $(a+b)^2 = a^2 + 2ab + b^2$:
\[(1 - \sqrt{1 - \frac{l - 4}{k}})^2 + (1 + \sqrt{1 - \frac{l - 4}{k}})^2 = 2 + 2(1 - \frac{l - 4}{k})(1 - \frac{l - 4}{k}) = 2 + 2(1 - \frac{2(l - 4)}{k} + \frac{(l - 4)^2}{k^2}).\]

So the sum of the squares of the distances from $A$ and $B$ to the origin is:
\[2 + 2(1 - \frac{2(l - 4)}{k} + \frac{(l - 4)^2}{k^2}) + 32 = 34 + 2(1 - \frac{2(l - 4)}{k} + \frac{(l - 4)^2}{k^2}).\]

This is a complicated expression, but we can simplify it further by using the condition that the line $y = 4$ is tangent to the parabola $y = kx^2 - 2kx + l$. This means that the discriminant of equation (1) is zero:
\[(2k)^2 - 4k(l - 4) = 0.\]
Simplifying, we get:
\[4k^2 - 4k(l - 4) = 0,\]
\[4k^2 - 4kl + 16k = 0,\]
\[k^2 - kl + 4k = 0.\]

We can solve this equation for $l$ in terms of $k$:
\[l = k + \frac{4k}{k} = k + 4.\]

Substituting this into our expression for the sum of the squares of the distances, we get:
\[34 + 2(1 - \frac{2((k + 4) - 4)}{k} + \frac{((k + 4) - 4)^2}{k^2}) = 34 + 2(1 - \frac{2k}{k} + \frac{k^2}{k^2}) = 34 + 2(1 - 2 + 1) = 34.\]

Therefore, the sum of the squares of the distances from $A$ and $B$ to the origin is 34. The answer is: $34$

BOXED []
BOXED FINAL 34
eval() arg 1 must be a string, bytes or code object final_eval
[(52, 1), (12, 1), (34, 1)]
code_answers 0 text_answers 3



## QUESTION 0 - 4 
- TIME_SPENT : 0 secs

4_User:

Below is a math problem you are to solve (positive numerical answer!):
"Let $k, l > 0$ be parameters. The parabola $y = kx^2 - 2kx + l$ intersects the line $y = 4$ at two points $A$ and $B$. These points are distance 6 apart. What is the sum of the squares of the distances from $A$ and $B$ to the origin?"
Analyze this problem and think step by step to come to a solution with programs. After solving the problem, output the final numerical answer within \boxed{}.

Assistant:

 To solve this problem, we first need to find the $x$-coordinates of points $A$ and $B$. We can do this by setting $y = 4$ in the equation of the parabola and solving for $x$.

```python


INTERMEDIATE OUT :

from sympy import symbols, Eq, solve

def find_x_coordinates():
    x, k, l = symbols('x k l')
    y = k*x**2 - 2*k*x + l

    # Set y = 4
    equation = Eq(y, 4)

    # Solve for x
    solutions = solve(equation, x)

    return solutions

solutions = find_x_coordinates()
print(solutions)
```

CODE RESULTS [(k - sqrt(k*(k - l + 4)))/k, (k + sqrt(k*(k - l + 4)))/k]

INTERMEDIATE OUT :
```output
[(k - sqrt(k*(k - l + 4)))/k, (k + sqrt(k*(k - l + 4)))/k]
```
The $x$-coordinates of points $A$ and $B$ are $\left(\frac{k - \sqrt{k(k - l + 4)}}{k}\right)$ and $\left(\frac{k + \sqrt{k(k - l + 4)}}{k}\right)$ respectively.

The distance between $A$ and $B$ is given as 6. Therefore, we have
\[AB = \left|\frac{k + \sqrt{k(k - l + 4)}}{k} - \frac{k - \sqrt{k(k - l + 4)}}{k}\right| = \frac{2\sqrt{k(k - l + 4)}}{k} = 6.\]
Squaring both sides, we get
\[\frac{4k(k - l + 4)}{k^2} = 36.\]
Simplifying, we have
\[4(k - l + 4) = 36k.\]
\[4k - 4l + 16 = 36k.\]
\[-4l + 16 = 32k.\]
\[-4l = 32k - 16.\]
\[-l = 8k - 4.\]
\[l = 4 - 8k.\]

Now, we need to find the sum of the squares of the distances from $A$ and $B$ to the origin. The distance from a point $(x, y)$ to the origin $(0, 0)$ is given by $\sqrt{x^2 + y^2}$.

The $y$-coordinate of points $A$ and $B$ can be found by substituting the $x$-coordinates into the equation of the parabola.

The sum of the squares of the distances from $A$ and $B$ to the origin is then
\[(x_A^2 + y_A^2) + (x_B^2 + y_B^2).\]

Let's calculate this in Python:

```python


INTERMEDIATE OUT :

from sympy import symbols, sqrt

def calculate_distance_sum():
    k, l = symbols('k l')

    # x-coordinates of points A and B
    x_A = (k - sqrt(k*(k - l + 4)))/k
    x_B = (k + sqrt(k*(k - l + 4)))/k

    # y-coordinates of points A and B
    y_A = k*x_A**2 - 2*k*x_A + l
    y_B = k*x_B**2 - 2*k*x_B + l

    # Sum of the squares of the distances from A and B to the origin
    distance_sum = x_A**2 + y_A**2 + x_B**2 + y_B**2

    # Substitute l = 4 - 8k
    distance_sum = distance_sum.subs(l, 4 - 8*k)

    return distance_sum

distance_sum = calculate_distance_sum()
print(distance_sum)
```

CODE RESULTS (-10*k - 6*Abs(k) + 4 + (k + 3*Abs(k))**2/k)**2 + (-10*k + 6*Abs(k) + 4 + (k - 3*Abs(k))**2/k)**2 + (k - 3*Abs(k))**2/k**2 + (k + 3*Abs(k))**2/k**2

INTERMEDIATE OUT :
```output
(-10*k - 6*Abs(k) + 4 + (k + 3*Abs(k))**2/k)**2 + (-10*k + 6*Abs(k) + 4 + (k - 3*Abs(k))**2/k)**2 + (k - 3*Abs(k))**2/k**2 + (k + 3*Abs(k))**2/k**2
```
The expression obtained for the sum of the squares of the distances from $A$ and $B$ to the origin is quite complicated. However, we can simplify it by noting that the absolute value terms cancel out:

```python


INTERMEDIATE OUT :

from sympy import simplify

def simplify_distance_sum():
    distance_sum = calculate_distance_sum()
    simplified_distance_sum = simplify(distance_sum)
    return simplified_distance_sum

simplified_distance_sum = simplify_distance_sum()
print(simplified_distance_sum)
``````output

CODE RESULTS 52

INTERMEDIATE OUT :

52
```
So, the sum of the squares of the distances from $A$ and $B$ to the origin is $52$.
The answer is: $52$

BOXED []
BOXED FINAL 52
[(52, 3), (12, 1), (34, 1)]
GOOD ANSWER UPDATED!
code_answers 1 text_answers 4



## QUESTION 0 - 5 
- TIME_SPENT : 0 secs

5_User:

Below is a math problem you are to solve (positive numerical answer!):
"Let $k, l > 0$ be parameters. The parabola $y = kx^2 - 2kx + l$ intersects the line $y = 4$ at two points $A$ and $B$. These points are distance 6 apart. What is the sum of the squares of the distances from $A$ and $B$ to the origin?"
Analyze this problem and think step by step to come to a solution with programs. After solving the problem, output the final numerical answer within \boxed{}.

Assistant:

 To solve this problem, we first need to find the x-coordinates of points $A$ and $B$. Since the parabola $y = kx^2 - 2kx + l$ intersects the line $y = 4$, we can set these two equal to each other and solve for $x$.

```python


INTERMEDIATE OUT :

from sympy import symbols, Eq, solve

def find_x_coordinates():
    x, k, l = symbols('x k l')
    equation = Eq(k * x**2 - 2 * k * x + l, 4)
    solutions = solve(equation, x)
    return solutions

solutions = find_x_coordinates()
print(solutions)
```

CODE RESULTS [(k - sqrt(k*(k - l + 4)))/k, (k + sqrt(k*(k - l + 4)))/k]

INTERMEDIATE OUT :
```output
[(k - sqrt(k*(k - l + 4)))/k, (k + sqrt(k*(k - l + 4)))/k]
```
Let's denote the x-coordinates of points $A$ and $B$ as $x_1$ and $x_2$ respectively. Then $x_1 = \frac{k - \sqrt{k(k - l + 4)}}{k}$ and $x_2 = \frac{k + \sqrt{k(k - l + 4)}}{k}$.

The distance between $A$ and $B$ is given as 6, so $|x_2 - x_1| = 6$. We can use this equation to solve for $l$ in terms of $k$.

```python


INTERMEDIATE OUT :

from sympy import symbols, solve, sqrt

def solve_for_l():
    k, l = symbols('k l')
    x1 = (k - sqrt(k*(k - l + 4)))/k
    x2 = (k + sqrt(k*(k - l + 4)))/k
    equation = Eq(abs(x2 - x1), 6)
    solution = solve(equation, l)
    return solution

solution = solve_for_l()
print(solution)
```

CODE RESULTS Traceback: line 1007, in solve
    raise NotImplementedError('solving %s when the argument '
NotImplementedError: solving Abs(sqrt(k**2 - k*l + 4*k)/k) when the argument is not real or imaginary.

FAIL


INTERMEDIATE OUT :
```output
Traceback: line 1007, in solve
    raise NotImplementedError('solving %s when the argument '
NotImplementedError: solving Abs(sqrt(k**2 - k*l + 4*k)/k) when the argument is not real or imaginary.

FAIL

```
It seems that we made a mistake in our calculations. Let's go back and check our work. We made a mistake in our equation for the distance between $A$ and $B$. The correct equation should be $(x_2 - x_1)^2 = 6^2$. Let's correct this and try again.

```python


INTERMEDIATE OUT :

from sympy import symbols, solve, sqrt

def solve_for_l():
    k, l = symbols('k l')
    x1 = (k - sqrt(k*(k - l + 4)))/k
    x2 = (k + sqrt(k*(k - l + 4)))/k
    equation = Eq((x2 - x1)**2, 6**2)
    solution = solve(equation, l)
    return solution

solution = solve_for_l()
print(solution)
``````output

CODE RESULTS [4 - 8*k]

INTERMEDIATE OUT :

[4 - 8*k]
```
So, $l = 4 - 8k$. Now, we need to find the sum of the squares of the distances from $A$ and $B$ to the origin. The distance from a point $(x, y)$ to the origin is $\sqrt{x^2 + y^2}$. For point $A$, this distance is $\sqrt{x_1^2 + (k x_1^2 - 2k x_1 + l)^2}$. Similarly, for point $B$, this distance is $\sqrt{x_2^2 + (k x_2^2 - 2k x_2 + l)^2}$.

Let's calculate the sum of the squares of these distances:

```python


INTERMEDIATE OUT :

from sympy import symbols, sqrt, simplify

def calculate_distance_sum():
    k, l, x1, x2 = symbols('k l x1 x2')
    l = 4 - 8 * k
    distance_A = sqrt(x1**2 + (k * x1**2 - 2 * k * x1 + l)**2)
    distance_B = sqrt(x2**2 + (k * x2**2 - 2 * k * x2 + l)**2)
    distance_sum = simplify((distance_A**2 + distance_B**2).subs({x1: (k - sqrt(k*(k - l + 4)))/k, x2: (k + sqrt(k*(k - l + 4)))/k}))
    return distance_sum

distance_sum = calculate_distance_sum()
print(distance_sum)
``````output

CODE RESULTS 52

INTERMEDIATE OUT :

52
```
The sum of the squares of the distances from $A$ and $B$ to the origin is 52. The answer is $\boxed{52}$.

BOXED ['52']
BOXED FINAL 52
[(52, 5), (12, 1), (34, 1)]
GOOD ANSWER UPDATED!
ANSWER FOUND!
Predicted best answer: {0: (52, 5)}

prompt correctness:[3, 0]
##Score: 115.47619047619047

## Self-Reflections

### Question 0 0 reflection:
None
### Question 0 1 reflection:
None
### Question 0 2 reflection:
None
### Question 0 3 reflection:
None
### Question 0 4 reflection:
None
### Question 0 5 reflection:
None
---
