Solving problem 4 ...



## QUESTION 4 - 0 
- TIME_SPENT : 485 secs

0_User:

Question (hint: positive numerical answer):
"A function $f: \mathbb N \to \mathbb N$ satisfies the following two conditions for all positive integers $n$:$f(f(f(n)))=8n-7$ and $f(2n)=2f(n)+1$. Calculate $f(100)$."
Please put your final solution into \boxed{}.

Step-by-step Solution:


To calculate $f(100)$, we need to first understand the function $f$.
We are given that $f(f(f(n)))=8n-7$.
We also know that $f(2n)=2f(n)+1$.

Let's start with $n=1$. From the second equation, we have $f(2)=2f(1)+1$.
But from the first equation, we know that $f(f(f(1)))=8(1)-7=1$.
So, $f(f(f(1)))=1$ implies that $f(f(1))=1$.
Since we know $f(2)=2f(1)+1$, and $f(f(1))=1$, we can substitute this into the second equation to get $2f(1)+1=1$, which implies that $f(1)=0$.

Now we can use the second equation again to find $f(2)=2f(1)+1=2(0)+1=1$.

Now we can find $f(f(2))=f(1)=0$.
And using the first equation $f(f(f(2)))=8(2)-7=9$, but we know $f(f(2))=0$, contradiction.
So, the second equation must be wrong. We should use the first equation instead. 

Let's start from $n=1$ again and set $n=f(1)=0$, then from the first equation, we have $f(f(f(0)))=8(0)-7=-7$.
But we know $f(f(f(0)))=f(f(1))=f(1)=0$. So, $-7=0$, contradiction.
So, the first equation must also be wrong. 

Actually, both equations seem to be incorrect.
Let's check the conditions again.
The first condition $f(f(f(n)))=8n-7$ is incorrect because when $n=1$, we have $f(f(f(1)))=1$, but from the first equation, we get $f(f(f(1)))=8(1)-7=1$, which means the first equation holds for $n=1$.

However, the second condition $f(2n)=2f(n)+1$ is incorrect because when $n=1$, we have $f(2)=f(2)$, which should be $2f(1)+1=2(0)+1=1$, so the second equation holds for $n=1$.

After careful examination, we find that the mistake is in the second condition.
Actually, the second equation should be $f(2n)=2f(n)$ because the $f(1)=0$ and $f(2)=1$ make the second equation consistent with the first equation.

So, the correct function $f$ is $f(n)=0$ for $n$ even, and $f(n)=1$ for $n$ odd.

Finally, we calculate $f(100)$. Since $100$ is even, we have $f(100)=0$. The solution is $\boxed{0}$.
The answer is: $0$.

BOXED ['0']
BOXED FINAL 0
eval() arg 1 must be a string, bytes or code object final_eval
[(0, 1)]
GOOD ANSWER UPDATED!
code_answers 0 text_answers 1



## QUESTION 4 - 1 
- TIME_SPENT : 485 secs

1_User:

Question (hint: positive numerical answer):
"A function $f: \mathbb N \to \mathbb N$ satisfies the following two conditions for all positive integers $n$:$f(f(f(n)))=8n-7$ and $f(2n)=2f(n)+1$. Calculate $f(100)$."
Please put your final solution into \boxed{}.

Step-by-step Solution:



Firstly, let's try to find $f(1)$. Using the second equation, we have $f(2) = 2f(1) + 1$. And applying the first equation to $f(2)$, we get $f(f(2)) = 8(2) - 7 = 9$. Since $f(f(f(1))) = 9$, we have $f(f(1)) = 8(1) - 7 = 1$ and then $f(1) = 1$.

Now let's try to find $f(2)$. Using the second equation, we have $f(4) = 2f(2) + 1$. And applying the first equation to $f(4)$, we get $f(f(4)) = 8(4) - 7 = 25$. Since $f(f(f(2))) = 25$, we have $f(f(2)) = 8(2) - 7 = 9$ and then $f(2) = 3$.

We can continue this process to find $f(3)$. Using the second equation, we have $f(6) = 2f(3) + 1$. And applying the first equation to $f(6)$, we get $f(f(6)) = 8(6) - 7 = 41$. Since $f(f(f(3))) = 41$, we have $f(f(3)) = 8(3) - 7 = 17$ and then $f(3) = 5$.

We can see a pattern here. It seems that $f(n) = 2n - 1$ for all positive integers $n$. Let's check if this pattern satisfies the two conditions of the problem.

For the first condition, $f(f(f(n))) = f(f(2n - 1)) = f(4n - 3) = 8(4n - 3) - 7 = 32n - 29$. And $8n - 7$. So we need to show that $32n - 29 = 8n - 7$. This simplifies to $32n - 8n = 22$, which is true. So the pattern holds for the first condition.

For the second condition, $f(2n) = f(4n - 2) = 8(4n - 2) - 7 = 32n - 17$, and $2f(n) + 1 = 2(2n - 1) + 1 = 4n - 1$. So we need to show that $32n - 17 = 4n - 1$. This simplifies to $32n - 4n = 16$, which is true. So the pattern holds for the second condition.

Therefore, the pattern $f(n) = 2n - 1$ holds for all positive integers $n$, and $f(100) = 2(100) - 1 = 199$. So the answer is $f(100) = \boxed{199}$.
The answer is: $199$

BOXED ['199']
BOXED FINAL 199
eval() arg 1 must be a string, bytes or code object final_eval
[(0, 1), (199, 1)]
code_answers 0 text_answers 2



## QUESTION 4 - 2 
- TIME_SPENT : 485 secs

2_User:

Question (hint: positive numerical answer):
"A function $f: \mathbb N \to \mathbb N$ satisfies the following two conditions for all positive integers $n$:$f(f(f(n)))=8n-7$ and $f(2n)=2f(n)+1$. Calculate $f(100)$."
Please put your final solution into \boxed{}.

Step-by-step Solution:



We are given that $f(f(f(n)))=8n-7$ and $f(2n)=2f(n)+1$. We want to find the value of $f(100)$.

Since we are asked to find $f(100)$, and we have a relation that involves $f(2n)$, it might be helpful to consider $200$ first, because $100$ is half of $200$. From the second relation, we have $f(200) = 2f(100) + 1$.

Now, we want to find $f(200)$, so we can use the first relation: $f(f(f(200))) = 8*200 - 7 = 1593$.

Since $f(f(f(200))) = f(f(2f(100)+1)) = f(2f(2f(100))+1)$, we can use the second relation again to get:

$f(2f(2f(100))+1) = 2f(f(2f(100))+1) + 1 = 1593$.

Let $x = f(100)$, then the equation becomes $f(2(2x+1)+1) = 1593$, or $f(4x+3) = 1593$.

However, we cannot directly find $f(100)$ from this equation, because it involves $f(4x+3)$.

Notice that if we take $n=1$ in the first relation $f(f(f(n)))=8n-7$, we get $f(f(f(1)))=8*1-7 = 1$. This means $f(f(1)) = 1$, because the function $f$ takes the number 1 to 1.

And if we take $n=1$ in the second relation $f(2n)=2f(n)+1$, we get $f(2)=2f(1)+1 = 2*1+1 = 3$. This means $f(2) = 3$, because the function $f$ takes the number 2 to 3.

Now we try $n=3$ in the second relation, we get $f(6)=2f(3)+1$. From the equation above, we know $f(6)=f(2*3)=f(2)*2+1 = 3*2+1 = 7$. So $f(6) = 7$.

If we take $n=7$ in the first relation, we get $f(f(f(7)))=8*7-7 = 56-7 = 49$. This means $f(f(7)) = 49$, because the function $f$ takes the number 7 to 49.

If we take $n=7$ in the second relation, we get $f(14)=2f(7)+1 = 2*49+1 = 99$. This means $f(14) = 99$.

We found $f(1)=1$, $f(2)=3$, $f(3)=5$, $f(6)=7$, $f(7)=49$, $f(14)=99$. Then we can use these to find $f(4x+3)$:

$f(4x+3) = f(4*1+3) = f(7) = 49$, for $x=1$.

$f(4x+3) = f(4*2+3) = f(11)$, but from the second relation, we know $f(11) = 2f(5.5)$ which does not help us.

$f(4x+3) = f(4*3+3) = f(15)$, but from the second relation, we know $f(15) = 2f(7.5)$ which does not help us.

$f(4x+3) = f(4*7+3) = f(31)$, but from the second relation, we know $f(31) = 2f(15.5)$ which does not help us.

However, we can use the fact that $f(14) = 99$ to find $f(31)$: from the second relation, we have $f(31) = 2f(15.5) = 2(f(14)*2+1) = 2(99*2+1) = 2*199 = 398$. So $f(31) = 398$.

Thus, $f(4x+3) = 398$ for $x=7$.

We found $f(4x+3) = 398$ for $x=7$, so we can write $f(4*7+3) = 398$. This means $f(31) = 398$.

Therefore, we have $f(2f(100)+1) = 1593$, which gives us $f(2x+1) = 1593/2 = 796.5$.

However, we know that $f(2x+1)$ must be an integer, so there must be a mistake in our reasoning.

Let's start again with a different approach. We know that $f(f(f(n)))=8n-7$, so if we take $n=1$, we get $f(f(f(1)))=8*1-7=1$, so $f(f(1))=1$.

Then if we take $n=2$, we get $f(f(f(2)))=8*2-7=9$.

From $f(f(1))=1$, we can see that $f(1)=1$.

Now if we substitute $n=1$ into the equation $f(2n)=2f(n)+1$, we get $f(2)=2f(1)+1=3$. So $f(2)=3$.

Then if we substitute $n=2$ into the equation $f(2n)=2f(n)+1$, we get $f(4)=2f(2)+1=7$. So $f(4)=7$.

Now if we substitute $n=7$ into the equation $f(f(f(n)))=8n-7$, we get $f(f(f(7)))=8*7-7=56-7=49$. So $f(f(7))=49$.

Since we know that $f(7)=49$, we have $f(f(7))=49$.

Now if we substitute $n=14$ into the equation $f(2n)=2f(n)+1$, we get $f(28)=

BOXED []
BOXED FINAL 
eval() arg 1 must be a string, bytes or code object final_eval
[(0, 1), (199, 1)]
code_answers 0 text_answers 2



## QUESTION 4 - 3 
- TIME_SPENT : 485 secs

3_User:

Question (hint: positive numerical answer):
"A function $f: \mathbb N \to \mathbb N$ satisfies the following two conditions for all positive integers $n$:$f(f(f(n)))=8n-7$ and $f(2n)=2f(n)+1$. Calculate $f(100)$."
Please put your final solution into \boxed{}.

Step-by-step Solution:


To find $f(100)$, we first need to use the second equation of the function $f$. We know that $f(2n)=2f(n)+1$. 

Let's apply this equation to find $f(100)$. We can write $100 = 2 \cdot 50$, so
\[f(100) = 2f(50) + 1.\]

Now we need to find $f(50)$. Using the same equation $f(2n)=2f(n)+1$, we can write $50 = 2 \cdot 25$, so
\[f(50) = 2f(25) + 1.\]

We need to continue this process until we reach a value of $n$ for which we know the value of $f(n)$.

Let's continue this process:
\[f(25) = 2f(12.5) + 1.\]

But we know that $f$ is only defined for natural numbers (positive integers), and $12.5$ is not a natural number. So, we must have made a mistake somewhere. 

Let's go back and look at the first equation of the function $f$: $f(f(f(n)))=8n-7$. 

We can try to use this equation to find the value of $f(100)$. If we let $n=1$, we get
\[f(f(f(1)))=8 \cdot 1 - 7 = -1.\]
But a function value cannot be negative. So, we must have made a mistake in our previous steps. Let's go back and revise our steps.

Let's start over:
\[f(100) = 2f(50) + 1.\]
We can use the second equation again to find $f(50)$:
\[f(50) = 2f(25) + 1.\]
And we can use the second equation again to find $f(25)$:
\[f(25) = 2f(12.5) + 1.\]
But this time, let's use the first equation of the function $f$: $f(f(f(n)))=8n-7$. 

If we let $n=12.5$, we get
\[f(f(f(12.5)))=8 \cdot 12.5 - 7 = 80 - 7 = 73.\]
But we also know that $f(f(f(n)))=8n-7$, so
\[f(f(f(12.5))) = 8 \cdot 12.5 - 7 = 73.\]
Setting these two equal to each other, we get
\[f(f(f(12.5))) = f(f(f(12.5))) = 73.\]
This means that we must have made an error somewhere in our previous steps. Let's go back and revise our steps again.

Let's start over again and try a different approach.

If we look at the second equation of the function $f$: $f(2n)=2f(n)+1$, we can see that it involves doubling $f(n)$ and adding 1. This suggests that $f(n)$ might be odd for odd values of $n$. Let's test this by looking at the first equation of the function $f$: $f(f(f(n)))=8n-7$. 

If we let $n=1$, we get
\[f(f(f(1)))=8 \cdot 1 - 7 = -1.\]
But we know that $f(f(f(1)))$ must be a positive number (since $f$ is defined for positive integers), so our initial assumption that $f(n)$ is odd for odd values of $n$ is correct.

Now, let's try to find a pattern in the function $f$. From the second equation, we can see that if $n$ is even, then $f(n)$ is also even. And if $n$ is odd, then $f(n)$ is odd.

Let's try to apply this pattern to find $f(100)$. Since $100$ is even, we know that $f(100)$ must be even. The only even value that we haven't used yet is $2f(50) + 1$. If $f(50)$ is odd, then $2f(50) + 1$ will be odd, which is not possible because $f(100)$ must be even. So, we must have made a mistake in our previous steps.

Let's go back and revise our steps once more.

If we look at the first equation of the function $f$: $f(f(f(n)))=8n-7$, we can see that it involves subtracting 7 from $8n$. This suggests that $f(n)$ might be one less than a multiple of 8 for certain values of $n$. Let's test this by looking at the second equation of the function $f$: $f(2n)=2f(n)+1$.

If we let $n=1$, we get
\[f(2 \cdot 1) = 2f(1) + 1 \Rightarrow f(2) = 2f(1) + 1.\]
This means that if $f(1)$ is one less than a multiple of 8, then $f(2)$ will also be one less than a multiple of 8. Let's test this for $n=2$:
\[f(f(f(2)))=8 \cdot 2 - 7 = 9.\]
If $f(2)$ is one less than a multiple of 8, then $f(f(f(2)))$ should also be one less than a multiple of 8. Since $9$ is one less than $10$, this suggests that our assumption is correct.

Now, let's try to apply this pattern to find $f(100)$. Since $100$ is a multiple of $4$, we know that $f(100)$ must be one less than a multiple of $8$. The only such value that we haven't used yet is $8k - 1$, where $k$ is a positive integer. So, we can write
\[f(100) = 8k - 1.\]
Now, let's try to find the value of $k$. Since $100 = 2 \cdot 50$, we can use the second equation of the function $f$: $f(2n)=2f(n)+1$ to find $f(100)$:
\[f(100) = 2f(50) + 1.\]
We can use the second equation again to find $f(50)$:
\[f(50) = 2f(25) + 1.\]
And we can use the second equation again to find $f(

BOXED []
BOXED FINAL 
eval() arg 1 must be a string, bytes or code object final_eval
[(0, 1), (199, 1)]
code_answers 0 text_answers 2



## QUESTION 4 - 4 
- TIME_SPENT : 485 secs

4_User:

Question (hint: positive numerical answer):
"A function $f: \mathbb N \to \mathbb N$ satisfies the following two conditions for all positive integers $n$:$f(f(f(n)))=8n-7$ and $f(2n)=2f(n)+1$. Calculate $f(100)$."
Please put your final solution into \boxed{}.

Step-by-step Solution:


To find $f(100)$, we need to find the function $f$ defined by the two conditions $f(f(f(n)))=8n-7$ and $f(2n)=2f(n)+1$.

First, let's use the second condition to find $f(100)$. We want to express 100 as $2n$ for some positive integer $n$. We can see that $100 = 2 \cdot 50$. So we can use the second condition $f(2n)=2f(n)+1$ to find $f(100)$:
$$f(100) = f(2 \cdot 50) = 2f(50) + 1.$$

Now we need to find $f(50)$. Again, we can express 50 as $2 \cdot 25$, and apply the second condition:
$$f(50) = f(2 \cdot 25) = 2f(25) + 1.$$

Next, we need to find $f(25)$. Expressing 25 as $2 \cdot 12.5$ would not help us, because 12.5 is not an integer. However, we notice that $25 = f(12)$, because $f(f(f(12)))=8 \cdot 12 - 7 = 95$ and $f(2 \cdot 12) = 2f(12) + 1$, so $f(24) = 2f(12) + 1$. And we know that $f(f(f(12)))=95$, so $f(24) = 95$. Therefore, $f(25) = f(13)$, because $f(2 \cdot 13) = 2f(13) + 1$, so $f(26) = 2f(13) + 1$.

Next, we can use the first condition $f(f(f(n)))=8n-7$ to find $f(12)$, $f(13)$, and $f(26)$:
$$f(12) = 1, \quad f(13) = 5, \quad f(26) = 9.$$

Now we can substitute these values back into the previous equations to find $f(50)$ and $f(100)$:
$$f(50) = 2f(25) + 1 = 2f(13) + 1 = 2 \cdot 5 + 1 = 11,$$
$$f(100) = 2f(50) + 1 = 2 \cdot 11 + 1 = 23.$$

So the value of $f(100)$ is 23. The answer is: $23$

BOXED []
BOXED FINAL 23
eval() arg 1 must be a string, bytes or code object final_eval
[(0, 1), (199, 1), (23, 1)]
code_answers 0 text_answers 3



## QUESTION 4 - 5 
- TIME_SPENT : 485 secs

5_User:

Question (hint: positive numerical answer):
"A function $f: \mathbb N \to \mathbb N$ satisfies the following two conditions for all positive integers $n$:$f(f(f(n)))=8n-7$ and $f(2n)=2f(n)+1$. Calculate $f(100)$."
Please put your final solution into \boxed{}.

Step-by-step Solution:


To solve this problem, we need to apply the given conditions step by step.
First, let's use the second condition $f(2n)=2f(n)+1$ to find $f(100)$.
Since $100 = 2 \times 50$, we can apply the second condition to get $f(100) = 2f(50)+1$.

Now, we need to find $f(50)$. Since $50 = 2 \times 25$, we can apply the second condition again to get $f(50) = 2f(25)+1$.

Continuing this process, we need to find $f(25)$. Since $25 = 5 \times 5$, we can apply the second condition once more to get $f(25) = 2f(5)+1$.

Next, we need to find $f(5)$. Since $5$ is a prime number, we cannot apply the second condition directly. However, we can use the first condition $f(f(f(n)))=8n-7$ with $n=5$. We get $f(f(f(5)))=8 \times 5 - 7 = 33$.

Now, let's find $f(f(5))$ by setting $n=5$ in the second condition. We get $f(10)=2f(5)+1$.

Similarly, let's find $f(10)$ by setting $n=5$ in the second condition again. We get $f(20)=2f(10)+1$.

Now, let's find $f(20)$ using the first condition $f(f(f(n)))=8n-7$. We get $f(f(f(5)))=8 \times 5 - 7 = 33$.

Now, we have a system of three equations:
1. $f(f(f(5)))=33$.
2. $f(10)=2f(5)+1$.
3. $f(20)=2f(10)+1$.

We can substitute the second equation into the third to get $f(20)=2(2f(5)+1)+1=4f(5)+3$. Now, we can substitute this into the first equation to get $f(f(f(5)))=33 \Rightarrow f(4f(5)+3)=33$.

We can solve this equation by trying different values for $f(5)$ and see if it gives us a solution that makes sense. After trying a few values, we find that $f(5)=3$ gives us $f(4f(5)+3)=f(15)=33$.

Now, we can substitute $f(5)=3$ into the second equation to get $f(10)=2f(5)+1=2(3)+1=7$.

Finally, we substitute $f(10)=7$ into the third equation to get $f(20)=2f(10)+1=2(7)+1=15$.

Now, we can substitute $f(20)=15$ into the first condition $f(f(f(5)))=8n-7$ to get $f(f(f(5)))=8 \times 5 - 7 = 33$. This gives us $f(f(15))=33$.

Since $f(15)=33$, we have $f(f(15))=33$. This confirms our previous solution.

So, we have found $f(5)=3$, $f(10)=7$, and $f(20)=15$.

Now, we can substitute these values back into the second condition to find $f(50)$, $f(100)$, etc.

$f(50)=2f(25)+1=2f(5 \times 5)+1=2(2f(5)+1)+1=2(2(3)+1)+1=2(7)+1=15$.

$f(100)=2f(50)+1=2(15)+1=31$.

Therefore, $f(100)=31$.

The answer is: $31$

BOXED []
BOXED FINAL 31
eval() arg 1 must be a string, bytes or code object final_eval
[(0, 1), (199, 1), (23, 1), (31, 1)]
code_answers 0 text_answers 4



## QUESTION 4 - 6 
- TIME_SPENT : 485 secs

6_User:

Question (hint: positive numerical answer):
"A function $f: \mathbb N \to \mathbb N$ satisfies the following two conditions for all positive integers $n$:$f(f(f(n)))=8n-7$ and $f(2n)=2f(n)+1$. Calculate $f(100)$."
Please put your final solution into \boxed{}.

Step-by-step Solution:


We can start by substituting $n = 1$ into the first equation, which gives $f(f(f(1)))=8(1)-7=1$. Since $f(f(f(1)))=1$, this means $f(1)$ is a number such that $f(f(f(1)))=1$. By trial and error, we can find that $f(1) = 1$, because if we substitute $f(1) = 1$ into the equation $f(f(f(1)))=1$, we get $f(1) = 1$, which is true.

Next, we substitute $n = 2$ into the second equation, which gives $f(4) = 2f(2) + 1$. We can use this equation to express $f(2)$ in terms of $f(4)$.

Then, substitute $f(2)$ into the first equation to get
\[f(f(f(2)))=8(2)-7=9.\]
Since $f(f(f(2)))=9$, we know $f(2)$ is a number such that $f(f(f(2)))=9$. By trial and error, we can find that $f(2) = 3$, because if we substitute $f(2) = 3$ into the equation $f(f(f(2)))=9$, we get $f(2) = 3$, which is true.

Next, substitute $f(2) = 3$ into the second equation to get $f(4) = 2(3) + 1 = 7$.

We can continue this process to find $f(3)$, $f(6)$, $f(12)$, etc., until we find a pattern. After some trials, we can find that $f(n) = 2n - 1$ for all positive integers $n$.

Now we can check if this pattern satisfies the original conditions:

1. For the first equation, $f(f(f(n)))=8n-7$, if $f(n) = 2n - 1$, then $f(f(f(n)))=f(f(2n-1))=f(4n-3)=8n-7$. So the first equation holds true for this pattern.

2. For the second equation, $f(2n)=2f(n)+1$, if $f(n) = 2n - 1$, then $f(2n)=2(2n-1)+1=4n-1=2f(n)+1$. So the second equation also holds true for this pattern.

Therefore, we have found a solution that satisfies both conditions: $f(n) = 2n - 1$. Now we can calculate $f(100)$:
\[f(100) = 2(100) - 1 = 200 - 1 = 199.\]
So, $f(100) = 199$. The answer is: $199$

BOXED []
BOXED FINAL 199
eval() arg 1 must be a string, bytes or code object final_eval
[(199, 2), (0, 1), (23, 1), (31, 1)]
GOOD ANSWER UPDATED!
code_answers 0 text_answers 5



## QUESTION 4 - 7 
- TIME_SPENT : 485 secs

7_User:

Question (hint: positive numerical answer):
"A function $f: \mathbb N \to \mathbb N$ satisfies the following two conditions for all positive integers $n$:$f(f(f(n)))=8n-7$ and $f(2n)=2f(n)+1$. Calculate $f(100)$."
Please put your final solution into \boxed{}.

Step-by-step Solution:


First, let's find $f(1)$. We plug in $n=1$ into the second condition: $f(2) = 2f(1) + 1$. From the first condition, we know that $f(f(f(1))) = 8(1) - 7 = -1$. Since $f(f(f(1))) = f(f(1))$ (by the second condition for $n=f(1)$), and $f(f(1)) = f(1)$ (by the second condition for $n=1$), we have $f(1) = -1$. Then, we plug $n=1$ into the second condition to get $f(2) = 2f(1) + 1 = 2(-1) + 1 = -1$. Again, by the second condition for $n=2$, we have $f(4) = 2f(2) + 1 = 2(-1) + 1 = -1$. Continuing this pattern, we see that $f(n) = -1$ for all positive integers $n$. Indeed, this function satisfies both conditions. Thus, $f(100) = -1$. The answer is: $\boxed{-1}$.

BOXED []
BOXED FINAL 1
eval() arg 1 must be a string, bytes or code object final_eval
[(199, 2), (0, 1), (23, 1), (31, 1), (1, 1)]
code_answers 0 text_answers 6
Predicted best answer: {0: (26, 1), 1: (200, 1), 2: (1, 3), 3: (256, 3), 4: (199, 2)}

prompt correctness:[2, 0]
##Score: 110.83333333333333

## Self-Reflections

### Question 4 0 reflection:
None
### Question 4 1 reflection:
None
### Question 4 2 reflection:
None
### Question 4 3 reflection:
None
### Question 4 4 reflection:
None
### Question 4 5 reflection:
None
### Question 4 6 reflection:
None
### Question 4 7 reflection:
None
---
