Solving problem 4 ...



## QUESTION 4 - 0 
- TIME_SPENT : 570 secs

0_User:

Below is a math problem you are to solve (natural number answer):
"A function $f: \mathbb N \to \mathbb N$ satisfies the following two conditions for all positive integers $n$:$f(f(f(n)))=8n-7$ and $f(2n)=2f(n)+1$. Calculate $f(100)$."
To accomplish this, first list the problem's constraints, conditions and related knowledge, and thens solve the problem step by step. Be clear so even an idiot can follow your instructions. After solving the problem, output the final numerical answer within \boxed{}.

Assistant:

 First, let's list the problem's constraints, conditions and related knowledge:

1. The function $f: \mathbb N \to \mathbb N$ satisfies the following two conditions for all positive integers $n$: $f(f(f(n)))=8n-7$ and $f(2n)=2f(n)+1$.
2. We are to calculate $f(100)$.

To solve this problem, we need to find a way to use the given conditions to find the value of $f(100)$.

Let's start by applying the second condition, $f(2n)=2f(n)+1$, to find $f(100)$. We can write $100 = 2 \cdot 50$, so we have:

$$f(100) = 2f(50) + 1.$$

Now we need to find the value of $f(50)$. We can use the second condition again, with $50 = 2 \cdot 25$, so:

$$f(50) = 2f(25) + 1.$$

Continuing this process, we need to find $f(25)$. We can write $25 = 2 \cdot 12 + 1$, so:

$$f(25) = 2f(12.5) + 1.$$

But $12.5$ is not a natural number, so we have gone astray. Let's try a different approach.

We know that $f(f(f(n)))=8n-7$. Let's set $n=100$, so we have:

$$f(f(f(100))) = 8 \cdot 100 - 7 = 793.$$

Now, we know that $f(100)$ is an input to the function $f$ that gets fed into the function $f$ again, and the result is $793$. So we can write:

$$f(f(f(100))) = f(f(100)) = 793.$$

Now we need to find $f(f(100))$, or $f(x)$ where $x = f(100)$. We know from the second condition that $f(2n) = 2f(n) + 1$. Let's set $n = x$, so:

$$f(2x) = 2f(x) + 1.$$

But we also know that $f(2x) = f(100)$, so we can substitute that into the equation:

$$f(100) = 2f(x) + 1.$$

Now we can substitute $f(x)$ with $100$ (since we are trying to find the value of $f(100)$), so:

$$f(100) = 2 \cdot 100 + 1 = 201.$$

However, this does not match the value of $793$ we got from $f(f(f(100)))$. Let's try another approach.

We know that $f(f(f(n)))=8n-7$. Let's set $n=50$, so we have:

$$f(f(f(50))) = 8 \cdot 50 - 7 = 393.$$

Now, we know that $f(50)$ is an input to the function $f$ that gets fed into the function $f$ again, and the result is $393$. So we can write:

$$f(f(f(50))) = f(f(50)) = 393.$$

Now we need to find $f(f(50))$, or $f(x)$ where $x = f(50)$. We know from the second condition that $f(2n) = 2f(n) + 1$. Let's set $n = x$, so:

$$f(2x) = 2f(x) + 1.$$

But we also know that $f(2x) = f(50)$, so we can substitute that into the equation:

$$f(50) = 2f(x) + 1.$$

Now we can substitute $f(x)$ with $f(50)$ (since we are trying to find the value of $f(50)$), so:

$$f(50) = 2f(50) + 1.$$

This equation does not have a solution for $f(50)$, so let's try another approach.

We know that $f(f(f(n)))=8n-7$. Let's set $n=25$, so we have:

$$f(f(f(25))) = 8 \cdot 25 - 7 = 193.$$

Now, we know that $f(25)$ is an input to the function $f$ that gets fed into the function $f$ again, and the result is $193$. So we can write:

$$f(f(f(25))) = f(f(25)) = 193.$$

Now we need to find $f(f(25))$, or $f(x)$ where $x = f(25)$. We know from the second condition that $f(2n) = 2f(n) + 1$. Let's set $n = x$, so:

$$f(2x) = 2f(x) + 1.$$

But we also know that $f(2x) = f(25)$, so we can substitute that into the equation:

$$f(25) = 2f(x) + 1.$$

Now we can substitute $f(x)$ with $f(25)$ (since we are trying to find the value of $f(25)$), so:

$$f(25) = 2f(25) + 1.$$

This equation does not have a solution for $f(25)$, so let's try another approach.

We know that $f(f(f(n)))=8n-7$. Let's set $n=12.5$, so we have:

$$f(f(f(12.5))) = 8 \cdot 12.5 - 7 = 93.$$

Now, we know that $f(12.5)$ is an input to the function $f$ that gets fed into the function $f$ again, and the result is $93$. So we can write:

$$f(f(f(12.5))) = f(f(12.5)) = 93.$$

Now we need to find $f(f(12.5))$, or $f(x)$ where $x = f(12.5)$. We know from the

BOXED []
BOXED FINAL 
eval() arg 1 must be a string, bytes or code object final_eval
code_answers 0 text_answers 0



## QUESTION 4 - 1 
- TIME_SPENT : 570 secs

1_User:

Below is a math problem you are to solve (natural number answer!):
"A function $f: \mathbb N \to \mathbb N$ satisfies the following two conditions for all positive integers $n$:$f(f(f(n)))=8n-7$ and $f(2n)=2f(n)+1$. Calculate $f(100)$."
Analyze the problem and think step by step to come to a solution with programs. After solving the problem, output the final numerical answer within \boxed{}.

Assistant:

 This problem is a bit tricky to solve directly. However, we can make an observation that might help us. If we plug in $n=1$ into the second equation, we get $f(2)=2f(1)+1$. Now, if we plug this into the first equation, we get $f(f(f(1)))=f(f(2))=f(2f(1)+1)=8*1-7=1$. So, we have found that $f(f(f(1)))=1$. This implies that $f(1)$ must be an integer such that when it is input into the function three times, it equals 1. The only such integer is 1 itself. So, $f(1)=1$. Now, we can use this information to find $f(100)$.

We know that $f(2n)=2f(n)+1$. If we plug in $n=50$, we get $f(100)=2f(50)+1$. But we also know that $f(f(f(50)))=8*50-7=393$. Since $f(1)=1$, we can keep applying the function $f$ until we reach 50. We find that $f(50)=31$. So, $f(100)=2*31+1=63$.

Therefore, $f(100)=63$. The answer is: $63$

BOXED []
BOXED FINAL 63
eval() arg 1 must be a string, bytes or code object final_eval
[(63, 1)]
GOOD ANSWER UPDATED!
code_answers 0 text_answers 1



## QUESTION 4 - 2 
- TIME_SPENT : 570 secs

2_User:

Below is a math problem you are to solve (natural number answer!):
"A function $f: \mathbb N \to \mathbb N$ satisfies the following two conditions for all positive integers $n$:$f(f(f(n)))=8n-7$ and $f(2n)=2f(n)+1$. Calculate $f(100)$."
Analyze the problem and think step by step to come to a solution with programs. After solving the problem, output the final numerical answer within \boxed{}.

Assistant:

 To solve this problem, we can start by applying the second condition of the function $f$ to the first equation $f(f(f(n)))=8n-7$. We can substitute $f(f(n))$ with $2f(n)+1$ from the second condition:
$$f(2f(f(n))+1)=8n-7.$$
Then, we substitute $f(n)$ with $2f(n)+1$ again:
$$f(2(2f(n)+1)+1)=8n-7.$$
Simplifying the equation, we get:
$$f(4f(n)+3)=8n-7.$$
Now, we apply the second condition again to get:
$$2f(4f(n)+3)+1=8n-7.$$
Simplifying the equation, we get:
$$2(8f(n)-7)+1=8n-7.$$
Expanding and simplifying, we get:
$$16f(n)-14+1=8n-7.$$
Combining like terms, we get:
$$16f(n)-13=8n-7.$$
Adding 13 to both sides, we get:
$$16f(n)=8n+6.$$
Dividing both sides by 2, we get:
$$8f(n)=4n+3.$$
Dividing both sides by 4, we get:
$$2f(n)=n+\frac{3}{2}.$$
But $f(n)$ is a natural number, so the right side of the equation cannot be a natural number unless $n=1$. Therefore, we can conclude that $f(1)=1$.
Now, we can use the second condition of the function $f$ to find $f(2)$:
$$f(2)=2f(1)+1=2(1)+1=3.$$
Similarly, we can find $f(3)$:
$$f(3)=2f(2)+1=2(3)+1=7.$$
Continuing this process, we can find that $f(n)=n$ for all positive integers $n$.
Therefore, $f(100)=100$.
The answer is: $100$

BOXED []
BOXED FINAL 100
eval() arg 1 must be a string, bytes or code object final_eval
[(63, 1), (100, 1)]
code_answers 0 text_answers 2



## QUESTION 4 - 3 
- TIME_SPENT : 570 secs

3_User:

Below is a math problem you are to solve (natural number answer!):
"A function $f: \mathbb N \to \mathbb N$ satisfies the following two conditions for all positive integers $n$:$f(f(f(n)))=8n-7$ and $f(2n)=2f(n)+1$. Calculate $f(100)$."
Analyze the problem and think step by step to come to a solution with programs. After solving the problem, output the final numerical answer within \boxed{}.

Assistant:

 This problem is a bit tricky to solve directly, but we can use the second equation to simplify it.

First, we can use the second equation to find $f(100)$. We know that $f(2n) = 2f(n) + 1$. So, if we let $n = 50$, we get $f(100) = 2f(50) + 1$.

Now, we can use the first equation to find $f(50)$. We know that $f(f(f(n))) = 8n - 7$. So, if we let $n = 25$, we get $f(f(f(25))) = 8*25 - 7 = 200 - 7 = 193$. But from the second equation, $f(f(f(25))) = f(f(50)) = f(100)$. So, we have $f(100) = 193$.

Then we can substitute $f(100) = 193$ into the equation $f(100) = 2f(50) + 1$ to find $f(50)$. We get $193 = 2f(50) + 1$, so $2f(50) = 193 - 1 = 192$, and $f(50) = 192/2 = 96$.

Finally, we can substitute $f(50) = 96$ into the equation $f(50) = 2f(25) + 1$ to find $f(25)$. We get $96 = 2f(25) + 1$, so $2f(25) = 96 - 1 = 95$, and $f(25) = 95/2 = 47.5$. But $f(25)$ must be a natural number, so there seems to be a mistake in our reasoning.

Let's try another approach. We know that $f(f(f(n))) = 8n - 7$. If we let $n = 1$, we get $f(f(f(1))) = 8*1 - 7 = 1$. So, $f(f(f(1))) = 1$.

Now, we know that $f(f(f(1))) = 1$, so $f(f(1)) = f(1)$. Then, we can substitute $n = 1$ into the second equation to get $f(2) = 2f(1) + 1$.

We also know that $f(f(1)) = f(1)$, so we can substitute $n = 1$ into the first equation to get $f(f(f(1))) = 8*1 - 7 = 1$, so $f(f(1)) = 1$. But we just showed that $f(f(1)) = f(1)$, so $f(1) = 1$.

Then, we can substitute $n = 1$ into the second equation to get $f(2) = 2f(1) + 1 = 2*1 + 1 = 3$.

Now, we can substitute $n = 2$ into the second equation to get $f(4) = 2f(2) + 1 = 2*3 + 1 = 7$.

Then, we can substitute $n = 4$ into the second equation to get $f(8) = 2f(4) + 1 = 2*7 + 1 = 15$.

We can continue this process, but it will be quite tedious. Instead, let's look for a pattern. We have $f(1) = 1$, $f(2) = 3$, $f(4) = 7$, $f(8) = 15$. It seems that $f(2^k) = 2^k - 1$ for all positive integers $k$.

Let's check this for $k = 5$. If $f(2^5) = 2^5 - 1$, then $f(32) = 31$. We can substitute $n = 16$ into the first equation to get $f(f(f(16))) = 8*16 - 7 = 128 - 7 = 121$. But from the second equation, $f(f(f(16))) = f(f(32)) = f(31)$. So, $f(31) = 121$. But we just showed that $f(32) = 31$, so $f(32) = 31$. This supports our pattern.

Now, we can use this pattern to find $f(50)$. Since $50 = 2*25 = 2^1*2^3*5$, we can use the second equation to find $f(50)$. We have $f(50) = 2f(25) + 1 = 2(2*12.5 + 1) + 1 = 2(25) + 1 = 51$.

Finally, we can substitute $f(50) = 51$ into the equation $f(100) = 2f(50) + 1$ to find $f(100)$. We get $f(100) = 2*51 + 1 = 103$.

So, the value of $f(100)$ is $103$. The answer is: $103$

BOXED []
BOXED FINAL 103
eval() arg 1 must be a string, bytes or code object final_eval
[(63, 1), (100, 1), (103, 1)]
code_answers 0 text_answers 3



## QUESTION 4 - 4 
- TIME_SPENT : 570 secs

4_User:

Below is a math problem you are to solve (natural number answer):
"A function $f: \mathbb N \to \mathbb N$ satisfies the following two conditions for all positive integers $n$:$f(f(f(n)))=8n-7$ and $f(2n)=2f(n)+1$. Calculate $f(100)$."
To accomplish this, first list the problem's constraints, conditions and related knowledge, and thens solve the problem step by step. Be clear so even an idiot can follow your instructions. After solving the problem, output the final numerical answer within \boxed{}.

Assistant:

 First, let's list the problem's constraints, conditions and related knowledge:

1. The function $f: \mathbb N \to \mathbb N$ satisfies the conditions $f(f(f(n)))=8n-7$ and $f(2n)=2f(n)+1$.
2. We are asked to calculate $f(100)$.

Now, let's solve the problem step by step:

We are given the equation $f(f(f(n)))=8n-7$. If we set $n=1$, we get $f(f(f(1)))=8*1-7=1$. Since $f(f(f(1)))=1$, and $f(1)$ is a natural number, we can conclude that $f(1)=1$.

Now, let's use the second equation $f(2n)=2f(n)+1$. If we set $n=1$, we get $f(2)=2f(1)+1=2*1+1=3$.

Now, let's use the first equation $f(f(f(n)))=8n-7$ again. If we set $n=2$, we get $f(f(f(2)))=8*2-7=9$. Since $f(f(f(2)))=9$, and we know that $f(2)=3$, we can substitute $f(2)$ into the equation to get $f(f(3))=9$.

Again, using the second equation $f(2n)=2f(n)+1$, if we set $n=3$, we get $f(6)=2f(3)+1$. But we know that $f(f(3))=9$, so we can substitute $f(3)$ into the equation to get $f(6)=2*9+1=19$.

Now, let's use the first equation $f(f(f(n)))=8n-7$ one more time. If we set $n=3$, we get $f(f(f(3)))=8*3-7=17$. Since $f(f(f(3)))=17$, and we know that $f(f(3))=9$, we can substitute $f(f(3))$ into the equation to get $f(9)=17$.

Finally, let's use the second equation $f(2n)=2f(n)+1$. If we set $n=9$, we get $f(18)=2f(9)+1=2*17+1=35$.

Now, let's use the first equation $f(f(f(n)))=8n-7$ one last time. If we set $n=9$, we get $f(f(f(9)))=8*9-7=65$. Since $f(f(f(9)))=65$, and we know that $f(18)=35$, we can substitute $f(18)$ into the equation to get $f(35)=65$.

But we are asked to find $f(100)$. Notice that $100$ is in the range of $f(n)$, specifically $f(35)=100$. Therefore, $f(100)=35$.

So, the value of $f(100)$ is $35$. The answer is: $35$.

BOXED []
BOXED FINAL 35
eval() arg 1 must be a string, bytes or code object final_eval
[(63, 1), (100, 1), (103, 1), (35, 1)]
code_answers 0 text_answers 4



## QUESTION 4 - 5 
- TIME_SPENT : 570 secs

5_User:

Below is a math problem you are to solve (natural number answer):
"A function $f: \mathbb N \to \mathbb N$ satisfies the following two conditions for all positive integers $n$:$f(f(f(n)))=8n-7$ and $f(2n)=2f(n)+1$. Calculate $f(100)$."
To accomplish this, first list the problem's constraints, conditions and related knowledge, and thens solve the problem step by step. Be clear so even an idiot can follow your instructions. After solving the problem, output the final numerical answer within \boxed{}.

Assistant:


To solve this problem, we need to use the given conditions to find the value of $f(100)$.

First, let's use the second condition $f(2n)=2f(n)+1$.
If we set $n=50$, we get $f(100)=2f(50)+1$.

Now, let's use the first condition $f(f(f(n)))=8n-7$.
If we set $n=50$, we get $f(f(f(50)))=8*50-7=393$.

Since $f(f(f(50)))=393$, we know that $f(50)$ is a number such that $f(f(f(50)))=f(50)=393$.
So, we need to find a number $x$ such that $f(f(x))=393$.

Again, using the first condition, we have $f(f(x))=8x-7$. Setting this equal to 393, we get $8x-7=393$, which simplifies to $8x=400$, or $x=50$.
So, $f(50)=50$.

Now, we can substitute $f(50)=50$ into the equation $f(100)=2f(50)+1$ to get $f(100)=2*50+1=101$.

So, $f(100)=101$. The answer is: $101$

BOXED []
BOXED FINAL 101
eval() arg 1 must be a string, bytes or code object final_eval
[(63, 1), (100, 1), (103, 1), (35, 1), (101, 1)]
code_answers 0 text_answers 5



## QUESTION 4 - 6 
- TIME_SPENT : 570 secs

6_User:

Below is a math problem you are to solve (natural number answer):
"A function $f: \mathbb N \to \mathbb N$ satisfies the following two conditions for all positive integers $n$:$f(f(f(n)))=8n-7$ and $f(2n)=2f(n)+1$. Calculate $f(100)$."
To accomplish this, first list the problem's constraints, conditions and related knowledge, and thens solve the problem step by step. Be clear so even an idiot can follow your instructions. After solving the problem, output the final numerical answer within \boxed{}.

Assistant:

 First, let's list the problem's constraints, conditions, and related knowledge:

1. The function $f: \mathbb N \to \mathbb N$ satisfies the conditions $f(f(f(n)))=8n-7$ and $f(2n)=2f(n)+1$ for all positive integers $n$.
2. We are to calculate $f(100)$.

To solve this problem, we will first try to find a pattern in the function $f(n)$ using the given conditions.

From the second condition, we have $f(2n)=2f(n)+1$. This implies that $f(n)$ is an increasing function.

Now, let's try to find $f(1)$ using the first condition. We have $f(f(f(1)))=8*1-7=1$. Since $f(f(f(1)))=1$, and $f(1)$ is a positive integer, we must have $f(1)=1$.

Now, using the second condition, we can find $f(2)=2f(1)+1=2*1+1=3$.

Similarly, we can find $f(4)=2f(2)+1=2*3+1=7$.

And, $f(8)=2f(4)+1=2*7+1=15$.

And, $f(16)=2f(8)+1=2*15+1=31$.

And, $f(32)=2f(16)+1=2*31+1=63$.

And, $f(64)=2f(32)+1=2*63+1=127$.

Now, let's check if $f(f(f(64)))=8*64-7=511$. We have $f(f(f(64)))=f(f(127))=f(255)$.

We can continue this process to find $f(511)$, but it will be very time-consuming. Instead, let's try to find a pattern in the values we have found.

We see that $f(2^n)=2^n-1$ for $n=1,2,3,4$. Let's check if this pattern holds for $n=5$. We have $f(32)=63$ and $32-1=63$, so the pattern holds for $n=5$.

Now, let's check if the first condition is satisfied for $n=64$. We have $f(f(f(64)))=f(f(127))=f(255)$. Using the pattern, we have $f(255)=255-1=254$. And, $8*64-7=511$. Since $254 \neq 511$, the pattern doesn't hold for all $n$.

However, we can notice that the pattern $f(2^n)=2^n-1$ holds for $n=1,2,3,4$, and the first condition is satisfied for these values. This suggests that the pattern might hold for all $n$ that are powers of 2.

Let's check if the pattern holds for $n=100$. Since $100$ is not a power of 2, we can't directly apply the pattern. However, we can use the second condition to find $f(100)$ indirectly.

We have $f(200)=2f(100)+1$. Using the pattern, we have $f(200)=200-1=199$. So, $2f(100)+1=199$, which gives $f(100)=\frac{199-1}{2}=99$.

So, the value of $f(100)$ is $99$. The answer is: $99$

BOXED []
BOXED FINAL 99
eval() arg 1 must be a string, bytes or code object final_eval
[(63, 1), (100, 1), (103, 1), (35, 1), (101, 1), (99, 1)]
code_answers 0 text_answers 6



## QUESTION 4 - 7 
- TIME_SPENT : 570 secs

7_User:

Below is a math problem you are to solve (natural number answer):
"A function $f: \mathbb N \to \mathbb N$ satisfies the following two conditions for all positive integers $n$:$f(f(f(n)))=8n-7$ and $f(2n)=2f(n)+1$. Calculate $f(100)$."
To accomplish this, first list the problem's constraints, conditions and related knowledge, and thens solve the problem step by step. Be clear so even an idiot can follow your instructions. After solving the problem, output the final numerical answer within \boxed{}.

Assistant:

 First, let's list the problem's constraints, conditions and related knowledge:

1. The function $f: \mathbb N \to \mathbb N$ satisfies the following two conditions for all positive integers $n$: $f(f(f(n)))=8n-7$ and $f(2n)=2f(n)+1$.
2. We are asked to calculate $f(100)$.

To solve this problem, we will first try to find a pattern in the function $f(n)$ by plugging in some small values of $n$ into the given conditions.

Let's start with the second condition: $f(2n)=2f(n)+1$.

If we plug in $n=1$, we get $f(2)=2f(1)+1$.
If we plug in $n=2$, we get $f(4)=2f(2)+1$.
If we plug in $n=3$, we get $f(6)=2f(3)+1$.
And so on.

From these equations, we can see that $f(n)$ is an odd function, as it increases by 1 when we double $n$.

Now let's try to use the first condition: $f(f(f(n)))=8n-7$.

If we plug in $n=1$, we get $f(f(f(1)))=8*1-7=1$.
So $f(f(1))=1$.

If we plug in $n=2$, we get $f(f(f(2)))=8*2-7=9$.
So $f(f(2))=9$.

If we plug in $n=3$, we get $f(f(f(3)))=8*3-7=17$.
So $f(f(3))=17$.

And so on.

From these equations, we can see that $f(n)$ is an increasing function, as it increases by 1, 9, 17, and so on, when we increase $n$ by 1, 2, and 3 respectively.

Now, let's try to find a pattern in the differences between consecutive values of $f(n)$.

The differences are: $f(2)-f(1)=7$, $f(4)-f(2)=8$, $f(6)-f(3)=16$, and so on.

From these differences, we can see that the differences are increasing by a factor of 2 each time.

So, we can conjecture that $f(n)=2^{n-1}+1$.

Now let's check if this conjecture satisfies the given conditions.

For the first condition, $f(f(f(n)))=8n-7$, let's plug in our conjecture:

$f(f(f(n)))=f(f(2^{n-1}+1))=f(2^{(2^{n-1}+1)-1}+1)=f(2^{2^{n-1}}+1)$.

And $8n-7=8(2^{n-1}+1)-7=2^{3+n-1}-7=2^{n+2}-7$.

So we need to show that $f(2^{2^{n-1}}+1)=2^{n+2}-7$.

Let $m=2^{2^{n-1}}+1$. Then $f(m)=2^{2^{n-1}+1}+1=2^{n+1}+1$.

And $2^{n+2}-7=2*2^{n+1}-7=2*(2^{n+1}+1)-9$.

So $f(m)=2^{n+1}+1=2^{n+2}-9$.

This does not hold true, so our conjecture is incorrect.

However, we can still use the second condition: $f(2n)=2f(n)+1$.

If we plug in $n=100$, we get $f(200)=2f(100)+1$.

And from the first condition: $f(f(f(100)))=8*100-7=793$.

So $f(f(f(100)))=793$.

Let's plug in $f(100)=x$ into the first condition: $f(f(f(100)))=f(f(x))=793$.

And from the second condition: $f(2x)=2f(x)+1=2x+1$.

So we need to solve the equation $f(2f(x)+1)=793$.

Let's plug in $f(x)=x$: $f(2x+1)=793$.

And from the second condition: $f(2x+1)=2f(x)+1=2x+1$.

So we have $2x+1=793$.

Solving for $x$, we get $x=\frac{793-1}{2}=396$.

So $f(100)=396$.

Therefore, the value of $f(100)$ is 396. The answer is: $396$

BOXED []
BOXED FINAL 396
eval() arg 1 must be a string, bytes or code object final_eval
[(63, 1), (100, 1), (103, 1), (35, 1), (101, 1), (99, 1), (396, 1)]
code_answers 0 text_answers 7
Predicted best answer: {0: (34, 2), 1: (0, 4), 2: (100, 2), 3: (100, 4), 4: (63, 1)}

prompt correctness:[0, 0]

## Self-Reflections

### Question 4 0 reflection:
None
### Question 4 1 reflection:
None
### Question 4 2 reflection:
None
### Question 4 3 reflection:
None
### Question 4 4 reflection:
None
### Question 4 5 reflection:
None
### Question 4 6 reflection:
None
### Question 4 7 reflection:
None
---
