Solving problem 4 ...



QUESTION 4 - 0 - TIME_SPENT : 497 secs
0_User: Below is a math problem you are to solve (positive numerical answer):
"A function $f: \mathbb N \to \mathbb N$ satisfies the following two conditions for all positive integers $n$:$f(f(f(n)))=8n-7$ and $f(2n)=2f(n)+1$. Calculate $f(100)$."
To accomplish this, first determine a sympy-based approach for solving the problem by listing each step to take and what functions need to be called in each step. Be clear so even an idiot can follow your instructions, and remember, your final answer should be positive integer, not an algebraic expression!
Write the entire script covering all the steps (use comments and document it well) and print the result. After solving the problem, output the final numerical answer within \boxed{}.

Approach:


To find $f(100)$, we can start by using the second given condition, $f(2n) = 2f(n) + 1$. 

If we apply this condition repeatedly, we can express $f(100)$ in terms of $f(50)$, $f(25)$, and so on. 

We also have the first given condition, $f(f(f(n))) = 8n - 7$. 

We can use this condition to express $f(n)$ in terms of $n$. 

For example, if we let $n = f(50)$, we have $f(f(f(50))) = 8*50 - 7 = 393$. 

So, $f(f(50)) = f(n) = \frac{393}{f(50)}$.

Now, we can use the second given condition to express $f(50)$ in terms of $f(25)$: $f(50) = 2f(25) + 1$. 

Similarly, we can express $f(25)$ in terms of $f(12.5)$: $f(25) = 2f(12.5) + 1$. 

But we have a problem here: the function $f$ is defined only for positive integers, so $f(12.5)$ is undefined. 

To get around this, we can use the second given condition again to express $f(12.5)$ in terms of $f(6.25)$: $f(12.5) = 2f(6.25) + 1$. 

And we can continue this process until we reach the base case, which is $f(1)$. 

For the base case, we can use the first given condition to find $f(1)$: $f(f(f(1))) = 8*1 - 7 = 1$. 

So, $f(f(1)) = f(n) = 1$, and thus $f(1) = 1$. 

Now we can work our way back up:

$f(6.25) = 2f(3.125) + 1$. 

Since $3.125$ is not an integer, we can continue the process until we reach $f(1)$, which we know is $1$. 

By working our way back up, we can find $f(6.25)$, $f(12.5)$, $f(25)$, and finally $f(50)$. 

Once we have $f(50)$, we can use the equation $f(50) = 2f(25) + 1$ to find $f(25)$. 

And then we can use the equation $f(25) = 2f(12.5) + 1$ to find $f(12.5)$. 

And finally, we can use the equation $f(12.5) = 2f(6.25) + 1$ to find $f(6.25)$. 

Then, we can use the equation $f(50) = 2f(25) + 1$ to find $f(50)$. 

Once we have $f(50)$, we can use the equation $f(100) = 2f(50) + 1$ to find $f(100)$. 

Here is the entire script:

```python


INTERMEDIATE OUT :

# Here is the sympy-based approach for solving the problem:

def find_f_100():
    # Base case: f(1) = 1
    f_1 = 1

    # Work our way up to f(6.25), f(12.5), f(25), f(50)
    # ...

    # Find f(50)
    f_50 = 2 * f_25 + 1

    # Find f(100)
    f_100 = 2 * f_50 + 1

    return f_100

result = find_f_100()
print(result)
```

name 'f_25' is not defined
FAIL

CODE RESULTS name 'f_25' is not defined
Try checking the formatting and imports

INTERMEDIATE OUT :
```output
name 'f_25' is not defined
Try checking the formatting and imports
```

The error in the code is that the values of $f(6.25)$, $f(12.5)$, and $f(25)$ are not defined. This is because the function $f$ is only defined for positive integers, not for decimal numbers. The approach we used here is not correct. 

However, we can notice that the function $f(f(f(n))) = 8n - 7$ is an extremely complicated function. It's not clear how to find $f(100)$ using this function directly. 

So, let's try another approach. We can use the second given condition $f(2n) = 2f(n) + 1$ repeatedly to find $f(100)$.

We have $f(100) = 2f(50) + 1$, $f(50) = 2f(25) + 1$, and $f(25) = 2f(12.5) + 1$. But we have a problem here again: the function $f$ is only defined for positive integers, so $f(12.5)$ is undefined. 

To get around this, we can use the second given condition to express $f(12.5)$ in terms of $f(6.25)$: $f(12.5) = 2f(6.25) + 1$. 

And we can continue this process until we reach the base case, which is $f(1)$. 

For the base case, we can use the first given condition to find $f(1)$: $f(f(f(1))) = 8*1 - 7 = 1$. 

So, $f(f(1)) = f(n) = 1$, and thus $f(1) = 1$. 

Now we can work our way back up:

$f(6.25) = 2f(3.125) + 1$. 

Since $3.125$ is not an integer, we can continue the process until we reach $f(1)$, which we know is $1$. 

By working our way back up, we can find $f(6.25)$, $f(12.5)$, $f(25)$, and finally $f(50)$. 

Once we have $f(50)$, we can use the equation $f(50) = 2f(25) + 1$ to find $f(25)$. 

And then we can use the equation $f(2

BOXED []
list index out of range
ERROR PARSING TEXT
invalid syntax (<string>, line 1) final_eval
code_answers 0 text_answers 0



QUESTION 4 - 1 - TIME_SPENT : 497 secs
1_User: Below is a math problem you are to solve (positive numerical answer!):
"A function $f: \mathbb N \to \mathbb N$ satisfies the following two conditions for all positive integers $n$:$f(f(f(n)))=8n-7$ and $f(2n)=2f(n)+1$. Calculate $f(100)$."
Analyze this problem and think step by step to come to a solution with programs. After solving the problem, output the final numerical answer within \boxed{}.



To solve this problem, we need to find the value of $f(100)$ based on the given conditions.

First, let's use the second condition $f(2n)=2f(n)+1$. We can substitute $n=50$ to get $f(100) = 2f(50)+1$.

Next, we need to find the value of $f(50)$. We can use the second condition again with $n=25$ to get $f(50) = 2f(25)+1$.

Similarly, we can find the value of $f(25)$ by using the second condition with $n=12.5$. However, $12.5$ is not a positive integer, so we cannot directly use the second condition here.

But we can use the first condition $f(f(f(n)))=8n-7$ with $n=25$. This gives us $f(f(f(25)))=8*25-7=193$.

Now we need to find the value of $f(f(25))$. We can use the second condition with $n=f(25)$ to get $f(f(25))=2f(f(12.5))+1$.

But we still cannot directly use the second condition with $n=12.5$. However, we can use the first condition with $n=12.5$. This gives us $f(f(f(12.5)))=8*12.5-7=93$.

Now we can substitute $f(f(12.5))=93$ into the equation $f(f(25))=2f(f(12.5))+1$ to get $f(f(25))=2*93+1=187$.

Finally, we can substitute $f(f(25))=187$ into the equation $f(50) = 2f(25)+1$ to get $f(50) = 2*187+1=375$.

Now we can substitute $f(50)=375$ into the equation $f(100) = 2f(50)+1$ to get $f(100) = 2*375+1=751$.

So the value of $f(100)$ is $751$. The answer is: $751$

BOXED []
list index out of range
ERROR PARSING TEXT
eval() arg 1 must be a string, bytes or code object final_eval
code_answers 0 text_answers 0



QUESTION 4 - 2 - TIME_SPENT : 497 secs
2_User: Below is a math problem you are to solve (positive numerical answer):
"A function $f: \mathbb N \to \mathbb N$ satisfies the following two conditions for all positive integers $n$:$f(f(f(n)))=8n-7$ and $f(2n)=2f(n)+1$. Calculate $f(100)$."
To accomplish this, first determine a sympy-based approach for solving the problem by listing each step to take and what functions need to be called in each step. Be clear so even an idiot can follow your instructions, and remember, your final answer should be positive integer, not an algebraic expression!
Write the entire script covering all the steps (use comments and document it well) and print the result. After solving the problem, output the final numerical answer within \boxed{}.

Approach:


The first step is to find a value for $f(1)$ using the second condition of the problem. Since $f(2n) = 2f(n) + 1$, we can set $n = 1$ to get $f(2) = 2f(1) + 1$. But we also know that $f(f(f(1))) = 8(1) - 7 = -1$, and since $f(f(f(1))) = f(f(x))$ for some $x$, we can set $x = 1$ to get $f(f(1)) = -1$. Now we can substitute $f(2)$ into the equation $f(f(1)) = -1$ to get $f(2) = -1$. Then we can substitute $f(2)$ into the equation $f(2) = 2f(1) + 1$ to get $-1 = 2f(1) + 1$, and solving for $f(1)$ gives $f(1) = -1$.

The second step is to use the value of $f(1)$ to find $f(2)$ using the second condition of the problem. We already found that $f(2) = 2f(1) + 1 = 2(-1) + 1 = -1$. But we know that $f(f(f(1))) = -1$, and since $f(f(f(1))) = f(f(x))$ for some $x$, we can set $x = 1$ to get $f(f(1)) = -1$. Now we can substitute $f(1)$ into the equation $f(f(1)) = -1$ to get $f(f(1)) = -1$. Since $f(f(1)) = f(2)$, we have $f(2) = -1$.

The third step is to use the value of $f(2)$ to find $f(4)$ using the second condition of the problem. We have $f(2n) = 2f(n) + 1$, so setting $n = 2$ gives $f(4) = 2f(2) + 1 = 2(-1) + 1 = -1$.

The fourth step is to use the value of $f(4)$ to find $f(8)$ using the second condition of the problem. We have $f(2n) = 2f(n) + 1$, so setting $n = 4$ gives $f(8) = 2f(4) + 1 = 2(-1) + 1 = -1$.

The fifth step is to use the value of $f(8)$ to find $f(16)$ using the second condition of the problem. We have $f(2n) = 2f(n) + 1$, so setting $n = 8$ gives $f(16) = 2f(8) + 1 = 2(-1) + 1 = -1$.

The sixth step is to use the value of $f(16)$ to find $f(32)$ using the second condition of the problem. We have $f(2n) = 2f(n) + 1$, so setting $n = 16$ gives $f(32) = 2f(16) + 1 = 2(-1) + 1 = -1$.

The seventh step is to use the value of $f(32)$ to find $f(64)$ using the second condition of the problem. We have $f(2n) = 2f(n) + 1$, so setting $n = 32$ gives $f(64) = 2f(32) + 1 = 2(-1) + 1 = -1$.

The eighth step is to use the value of $f(64)$ to find $f(128)$ using the second condition of the problem. We have $f(2n) = 2f(n) + 1$, so setting $n = 64$ gives $f(128) = 2f(64) + 1 = 2(-1) + 1 = -1$.

The ninth step is to use the value of $f(128)$ to find $f(256)$ using the second condition of the problem. We have $f(2n) = 2f(n) + 1$, so setting $n = 128$ gives $f(256) = 2f(128) + 1 = 2(-1) + 1 = -1$.

The tenth step is to use the value of $f(256)$ to find $f(512)$ using the second condition of the problem. We have $f(2n) = 2f(n) + 1$, so setting $n = 256$ gives $f(512) = 2f(256) + 1 = 2(-1) + 1 = -1$.

The eleventh step is to use the value of $f(512)$ to find $f(1024)$ using the second condition of the problem. We have $f(2n) = 2f(n) + 1$, so setting $n = 512$ gives $f(1024) = 2f(512) + 1 = 2(-1) + 1 = -1$.

The twelfth step is to use the value of $f(1024)$ to find $f(2048)$ using the second condition of the problem. We have $f(2n) = 2f(n) + 1$, so setting $n = 1024$ gives $f(2048) = 2f(1024) + 1 = 2(-1) + 1 = -1$.

The thirteenth step is to use the value of $f(2048)$ to find $f(4096)$ using the second condition of the problem. We have $f(2n) = 2f(n) + 1$, so setting $n = 2048$ gives $f(4096) = 2f(2048) + 1 = 2(-1) + 1 = -1$.

The fourteenth step is to use the value of $f(4096)$ to find $f(8192)$ using the second condition of the problem. We have $f(2n) = 2f(n) + 1$, so setting $n = 4096$ gives $f(8192) = 2f(4096) + 1 = 2(-1) + 1 = -1$.

The fifteenth step is to use the value of $f(8192)$ to find $f(16384)$ using the second condition of the problem. We have

BOXED []
list index out of range
ERROR PARSING TEXT
eval() arg 1 must be a string, bytes or code object final_eval
code_answers 0 text_answers 0



QUESTION 4 - 3 - TIME_SPENT : 497 secs
3_User: Below is a math problem you are to solve (positive numerical answer):
"A function $f: \mathbb N \to \mathbb N$ satisfies the following two conditions for all positive integers $n$:$f(f(f(n)))=8n-7$ and $f(2n)=2f(n)+1$. Calculate $f(100)$."
To accomplish this, first determine a sympy-based approach for solving the problem by listing each step to take and what functions need to be called in each step. Be clear so even an idiot can follow your instructions, and remember, your final answer should be positive integer, not an algebraic expression!
Write the entire script covering all the steps (use comments and document it well) and print the result. After solving the problem, output the final numerical answer within \boxed{}.

Approach:


To solve this problem, we can use a recursive function to calculate $f(100)$. The function $f$ is defined by two equations, namely $f(f(f(n)))=8n-7$ and $f(2n)=2f(n)+1$. The first equation is a recursive one, so we can use it to find $f(100)$ by calculating $f(f(f(100)))$ first, then $f(f(f(f(f(f(100))))))$, and so on until we reach $f(100)$.

Step 1: Define a recursive function `f` that takes a positive integer `n` as input and returns the value of $f(n)$ using the given conditions.

Step 2: Calculate $f(f(f(100)))$ using the first equation.

Step 3: Calculate $f(f(f(f(f(f(100))))))$ using the first equation again.

Step 4: Continue this process until we reach $f(100)$.

Step 5: The value of $f(100)$ will be our final answer.

Here is the Python code to implement this approach:

```python


INTERMEDIATE OUT :

from sympy import symbols, Eq, solve

def f(n):
    if n % 2 == 0:
        return 2 * f(n // 2) + 1
    else:
        return (8 * n - 7) // f(f(f(n)))

f100 = f(100)
print(f100)
```

maximum recursion depth exceeded in comparison
FAIL

CODE RESULTS maximum recursion depth exceeded in comparison

INTERMEDIATE OUT :
```output
maximum recursion depth exceeded in comparison
```
The code above is not working because the recursive function `f` is not defined correctly. Let's correct the function and try again.

Corrected `f` function:

```python


INTERMEDIATE OUT :

def f(n):
    if n == 100:
        return f(f(f(100)))
    elif n % 2 == 0:
        return 2 * f(n // 2) + 1
    else:
        return (8 * n - 7) // f(f(f(n)))

f100 = f(100)
print(f100)
```

maximum recursion depth exceeded in comparison
FAIL

CODE RESULTS maximum recursion depth exceeded in comparison
REPEATED ERRORS
BOXED []
list index out of range
ERROR PARSING TEXT
invalid syntax (<string>, line 1) final_eval
code_answers 0 text_answers 0



QUESTION 4 - 4 - TIME_SPENT : 497 secs
4_User: Below is a math problem you are to solve (positive numerical answer!):
"A function $f: \mathbb N \to \mathbb N$ satisfies the following two conditions for all positive integers $n$:$f(f(f(n)))=8n-7$ and $f(2n)=2f(n)+1$. Calculate $f(100)$."
Analyze this problem and think step by step to come to a solution with programs. After solving the problem, output the final numerical answer within \boxed{}.



To solve this problem, we can use the second condition $f(2n)=2f(n)+1$. We know that $f(f(f(100)))=8*100-7=793$. We can start by finding $f(f(100))$ using the second condition. If $f(f(100))=x$, then $f(2x)=2f(x)+1=793$. Since $f(2x)=2f(x)+1$, we have $2f(x)+1=793$, so $2f(x)=792$ and $f(x)=396$.
Now we can find $f(100)$ using the same method. If $f(100)=y$, then $f(2y)=2f(y)+1=396$. So $2f(y)+1=396$, $2f(y)=395$, and $f(y)=197.5$. But $f(y)$ must be a natural number, so there seems to be a mistake in our reasoning.
Let's try another approach. We know that $f(f(f(100)))=793$, so $f(f(x))=793$ when $x=100$. If $f(f(x))=z$, then $f(2z)=2f(z)+1=793$. So $2f(z)+1=793$, $2f(z)=792$, and $f(z)=396$. Therefore, $f(100)=396$.
Now we can find $f(100)$ using the second condition $f(2n)=2f(n)+1$. If $f(100)=y$, then $f(200)=2f(100)+1=793$. But we know that $f(200)=793$ from the first condition $f(f(f(200)))=793$. Therefore, $2f(100)+1=793$, $2f(100)=792$, and $f(100)=396$.
Finally, we can find $f(100)$ using the second condition $f(2n)=2f(n)+1$. If $f(100)=y$, then $f(200)=2f(100)+1=793$. But we know that $f(200)=793$ from the first condition $f(f(f(200)))=793$. Therefore, $2f(100)+1=793$, $2f(100)=792$, and $f(100)=396$.
So $f(100)=396$. The answer is: $396$

BOXED []
list index out of range
ERROR PARSING TEXT
eval() arg 1 must be a string, bytes or code object final_eval
code_answers 0 text_answers 0



QUESTION 4 - 5 - TIME_SPENT : 497 secs
5_User: Below is a math problem you are to solve (positive numerical answer!):
"A function $f: \mathbb N \to \mathbb N$ satisfies the following two conditions for all positive integers $n$:$f(f(f(n)))=8n-7$ and $f(2n)=2f(n)+1$. Calculate $f(100)$."
Analyze this problem and think step by step to come to a solution with programs. After solving the problem, output the final numerical answer within \boxed{}.



This problem is quite complex and requires a deep understanding of the properties of the function $f$. The given equations provide some clues about the function's behavior, but it's not straightforward to directly compute $f(100)$ from these equations.

However, we can make an observation: if we substitute $n = 1$ into the second equation, we get $f(2) = 2f(1) + 1$. And if we substitute $n = f(1)$ into the first equation, we get $f(f(f(f(1)))) = 8f(1) - 7$. But from the first equation, we know that $f(f(f(1))) = f(f(2)) = f(2f(1) + 1)$. So we have $f(2f(1) + 1) = 8f(1) - 7$. Comparing this with the second equation, we can see that $f(2f(1) + 1) = f(2)$ and $8f(1) - 7 = 2f(f(1)) + 1$. This implies that $f(2) = 8f(1) - 6$, and further simplification gives $f(2) = 2(4f(1) - 3)$. This means that $f(1)$ must be 3, because $f(2) = 2f(1) + 1$ and $f(2) = 2(4f(1) - 3)$ give $2f(1) + 1 = 2(4f(1) - 3)$, which simplifies to $f(1) = 3$.

Now we can compute $f(100)$ by repeatedly applying the second equation. We have:

\[
\begin{align*}
f(100) &= f(2 \cdot 50) \\
&= 2f(50) + 1.
\end{align*}
\]

We can continue this process to find $f(50)$, $f(25)$, and so on, until we reach $f(1) = 3$. By doing this, we find:

\[
\begin{align*}
f(1) &= 3, \\
f(2) &= 2f(1) + 1 = 2 \cdot 3 + 1 = 7, \\
f(4) &= 2f(2) + 1 = 2 \cdot 7 + 1 = 15, \\
f(8) &= 2f(4) + 1 = 2 \cdot 15 + 1 = 31, \\
f(16) &= 2f(8) + 1 = 2 \cdot 31 + 1 = 63, \\
f(32) &= 2f(16) + 1 = 2 \cdot 63 + 1 = 127, \\
f(64) &= 2f(32) + 1 = 2 \cdot 127 + 1 = 255, \\
f(100) &= 2f(50) + 1 = 2f(2 \cdot 25) + 1 = 2(2f(25) + 1) + 1 = 2(2(2f(12.5) + 1) + 1) + 1 = 2(2(2(2f(6.25) + 1) + 1) + 1) + 1 = 2(2(2(2(2f(3.125) + 1) + 1) + 1) + 1) + 1 = 2(2(2(2(2(2f(1.5625) + 1) + 1) + 1) + 1) + 1) + 1) = 2(2(2(2(2(2 \cdot 3 + 1) + 1) + 1) + 1) + 1) + 1) = 2(2(2(2(2 \cdot 7 + 1) + 1) + 1) + 1) + 1 = 2(2(2(2 \cdot 15 + 1) + 1) + 1) + 1 = 2(2(2 \cdot 31 + 1) + 1) + 1 = 2(2 \cdot 63 + 1) + 1 = 2 \cdot 127 + 1 = 255.
\end{align*}
\]

So $f(100) = 255$. The answer is: $255$

BOXED []
list index out of range
ERROR PARSING TEXT
eval() arg 1 must be a string, bytes or code object final_eval
code_answers 0 text_answers 0



QUESTION 4 - 6 - TIME_SPENT : 497 secs
6_User: Below is a math problem you are to solve (positive numerical answer!):
"A function $f: \mathbb N \to \mathbb N$ satisfies the following two conditions for all positive integers $n$:$f(f(f(n)))=8n-7$ and $f(2n)=2f(n)+1$. Calculate $f(100)$."
Analyze this problem and think step by step to come to a solution with programs. After solving the problem, output the final numerical answer within \boxed{}.



To solve this problem, we can use the second condition to find $f(100)$ by first finding $f(50)$ and then $f(25)$.
We start with $f(25)$:
\[f(2 \cdot 25) = 2f(25) + 1 \implies f(50) = 2f(25) + 1.\]
Then we find $f(50)$:
\[f(2 \cdot 50) = 2f(50) + 1 \implies f(100) = 2f(50) + 1.\]
We can substitute the expression for $f(50)$ into this equation:
\[f(100) = 2(2f(25) + 1) + 1 = 4f(25) + 3.\]
Now we can substitute the expression for $f(25)$ from the first equation:
\[f(25) = f(f(f(25))) = 8 \cdot 25 - 7 = 193.\]
Finally, we can substitute this value into the equation for $f(100)$:
\[f(100) = 4 \cdot 193 + 3 = 772 + 3 = 775.\]
So, $f(100) = 775$. The answer is: $775$

BOXED []
list index out of range
ERROR PARSING TEXT
eval() arg 1 must be a string, bytes or code object final_eval
code_answers 0 text_answers 0



QUESTION 4 - 7 - TIME_SPENT : 497 secs
7_User: Below is a math problem you are to solve (positive numerical answer):
"A function $f: \mathbb N \to \mathbb N$ satisfies the following two conditions for all positive integers $n$:$f(f(f(n)))=8n-7$ and $f(2n)=2f(n)+1$. Calculate $f(100)$."
To accomplish this, first determine a sympy-based approach for solving the problem by listing each step to take and what functions need to be called in each step. Be clear so even an idiot can follow your instructions, and remember, your final answer should be positive integer, not an algebraic expression!
Write the entire script covering all the steps (use comments and document it well) and print the result. After solving the problem, output the final numerical answer within \boxed{}.

Approach:


1. We know that $f(f(f(n)))=8n-7$. Let's set $f(n) = x$. Then we have $f(x) = 8n - 7$.
2. We also know that $f(2n) = 2f(n) + 1$. Let's set $n = 1$. Then we have $f(2) = 2f(1) + 1$.
3. From $f(f(f(n)))=8n-7$, we can deduce that $f(x) = 8n - 7$ implies $f(8n - 7) = n$.
4. Now we want to find $f(100)$, we need to find $x$ such that $f(x) = 100$.
5. From $f(2n) = 2f(n) + 1$, we can deduce that $f(2) = 2f(1) + 1$.
6. We can start by finding $f(1)$ using the equation $f(2) = 2f(1) + 1$. Since we know $f(2)$, we can find $f(1)$ by solving the equation.
7. Once we have $f(1)$, we can find $x$ such that $f(x) = 100$ by solving the equation $f(x) = 8n - 7$.
8. Finally, we can find $f(100)$ by substituting $x$ into the equation $f(x) = 8n - 7$.

Now, let's write the entire script to find $f(100)$.

```python


INTERMEDIATE OUT :

from sympy import symbols, Eq, solve

def find_f_100():
    # f_1: value of f(1)
    f_1 = symbols('f_1')
    # f_2: value of f(2)
    f_2 = 2 * f_1 + 1

    # From f(2) = 2f(1) + 1 and f(f(f(n)))=8n-7, we have f(2) = 8 - 7 = 1
    # So f(2) = 1
    equation = Eq(f_2, 1)

    # Solve for f(1)
    solution = solve(equation, f_1)
    f_1_value = solution[0]

    # Now we want to find x such that f(x) = 100
    x = symbols('x')
    equation = Eq(8 * x - 7, 100)
    solution = solve(equation, x)
    x_value = solution[0]

    # Finally, we can find f(100) by substituting x into the equation f(x) = 8n - 7
    f_100 = 8 * x_value - 7

    return f_100

result = find_f_100()
print(result)
```

100

CODE RESULTS 100

INTERMEDIATE OUT :
```output
100
```
The value of $f(100)$ is 100. The answer is: $100$

BOXED []
list index out of range
ERROR PARSING TEXT
[(100, 1)]
GOOD ANSWER UPDATED!
code_answers 1 text_answers 0
Predicted best answer: {0: (130, 1), 1: (800, 4), 2: (99, 1), 3: (256, 2), 4: (100, 1)}

==sep==
